<?xml version="1.0" encoding="UTF-8"?>
<rdf:RDF 
    xmlns:alt="http://id.altlaw.org/terms/"
    xmlns:dcterms="http://purl.org/dc/terms/"
    xmlns:foaf="http://xmlns.com/foaf/0.1/"
    xmlns:owl="http://www.w3.org/2002/07/owl#"
    xmlns:rdf="http://www.w3.org/1999/02/22-rdf-syntax-ns#"
    xmlns:rdfs="http://www.w3.org/2000/01/rdf-schema#"
    xmlns:xsd="http://www.w3.org/2001/XMLSchema#">

  <owl:Ontology rdf:about="">
    <dcterms:title>AltLaw.org Vocabulary</dcterms:title>
    <dcterms:description>
      An RDF vocabulary for Semantic Web applications using data
      provided by AltLaw.org.  The classes and properties defined here
      are intended to supplement metadata vocabularies such as Dublin
      Core.
    </dcterms:description>
  </owl:Ontology>

  <rdfs:Class rdf:about="http://id.altlaw.org/terms/Decision">
    <rdfs:label>Decision</rdfs:label>
    <rdfs:comment>
      A single decision released by a court, which may resolve
      multiple cases and contain multiple writings.
    </rdfs:comment>
  </rdfs:Class>

  <rdfs:Class rdf:about="http://id.altlaw.org/terms/Writing">
    <rdfs:label>Writing</rdfs:label>
    <rdfs:comment>
      A single writing within a decision, such as a majority decision,
      concurrence, or dissent.  Not currently used by AltLaw, but
      defined in other vocabularies such as OAI4Courts.
    </rdfs:comment>
  </rdfs:Class>

  <rdfs:Class rdf:about="http://id.altlaw.org/terms/Court">
    <rdfs:label>Court</rdfs:label>
    <rdfs:comment>
      Any court.  Refines "foaf:Organization".
    </rdfs:comment>
    <rdfs:subClassOf rdf:resource="http://xmlns.com/foaf/0.1/Organization"/>
  </rdfs:Class>

  <rdf:Property rdf:about="http://id.altlaw.org/terms/court">
    <rdfs:label>court</rdfs:label>
    <rdfs:comment>
      The court which originated a decision.  Refines
      "dcterms:coverage".
    </rdfs:comment>
    <rdfs:domain rdf:resource="http://id.altlaw.org/terms/Decision"/>
    <rdfs:range rdf:resource="http://id.altlaw.org/terms/Court"/>
    <rdfs:subPropertyOf rdf:resource="http://purl.org/dc/terms/coverage">
  </rdf:Property>
  
  <rdf:Property rdf:about="http://id.altlaw.org/terms/docket">
    <rdfs:label>docket</rdfs:label>
    <rdfs:comment>
      The docket number associated with a case or decision.  A single
      case or decision may have multiple docket numbers attached to
      it.  The range of this property is any string, which may include
      punctuation such as hyphens, but it should be a single docket
      number rather than a series such as "10-102; 10-103".  The
      string also should not contain abbreviations for "Number" such
      as "No." or "Nos.".  Refines "dcterms:identifier".
    </rdfs:comment>
    <rdfs:subPropertyOf rdf:resource="http://purl.org/dc/terms/identifier"/>
    <rdfs:range rdf:resource="http://www.w3.org/2000/01/rdf-schema#Literal"/>
  </rdf:Property>

  <rdf:Property rdf:about="http://id.altlaw.org/terms/bluebookIdentifier">
    <rdfs:label>Bluebook identifier</rdfs:label>
    <rdfs:comment>
      A citation to a decision in the form described by "A Uniform
      System of Citation", a.k.a. the Bluebook, available at
      http://www.legalbluebook.com/.  Values of this property should
      contain only the minimal information needed to identify the
      decision within a single publication, e.g. "123 F.3d 456".  They
      are not, therefore, complete citations as described by the
      Bluebook.  A single value of this property must not include
      parallel citations, but a single decision may have multiple
      bluebookIdentifiers, one for each parallel citation.  Refines
      "dcterms:identifier".
    </rdfs:comment>
    <rdfs:subPropertyOf rdf:resource="http://purl.org/dc/terms/identifier"/>
    <rdfs:domain rdf:resource="http://id.altlaw.org/terms/Decision"/>
    <rdfs:range rdf:resource="http://www.w3.org/2000/01/rdf-schema#Literal"/>
  </rdf:Property>

  <rdf:Property rdf:about="http://id.altlaw.org/terms/precedential">
    <rdfs:label>precedential</rdfs:label>
    <rdfs:comment>
      Boolean indicating whether or not a decision is considered
      "precedential" (or, equivalently, "published") by the court
      that issued it.
    </rdfs:comment>
    <rdfs:domain rdf:resource="http://id.altlaw.org/terms/Decision"/>
    <rdfs:range rdf:resource="http://www.w3.org/2000/01/rdf-schema#Literal"/>
  </rdf:Property>
</rdf:RDF>
