<?xml version="1.0" encoding="UTF-8"?>
<!DOCTYPE rdf:RDF [
    <!ENTITY alt "http://id.altlaw.org/terms/">
    <!ENTITY bibo "http://purl.org/ontology/bibo/">
    <!ENTITY dc "http://purl.org/dc/elements/1.1/">
    <!ENTITY dcterms "http://purl.org/dc/terms/">
    <!ENTITY foaf "http://xmlns.com/foaf/0.1/">
    <!ENTITY owl "http://www.w3.org/2002/07/owl#">
    <!ENTITY rdf "http://www.w3.org/1999/02/22-rdf-syntax-ns#">
    <!ENTITY rdfs "http://www.w3.org/2000/01/rdf-schema#">
    <!ENTITY xsd "http://www.w3.org/2001/XMLSchema#">
    <!ENTITY vann "http://purl.org/vocab/vann/">
    <!ENTITY dcdoc "http://dublincore.org/documents/dcmi-terms/">
    <!ENTITY nfo "http://www.semanticdesktop.org/ontologies/2007/03/22/nfo#">
    <!ENTITY nie "http://www.semanticdesktop.org/ontologies/2007/01/19/nie#">
]>
<rdf:RDF 
    xmlns:alt="&alt;"
    xmlns:bibo="&bibo;"
    xmlns:dcterms="&dcterms;"
    xmlns:foaf="&foaf;"
    xmlns:owl="&owl;"
    xmlns:nfo="&nfo;"
    xmlns:rdf="&rdf;"
    xmlns:rdfs="&rdfs;"
    xmlns:xsd="&xsd;"
    xmlns:vann="&vann;">


  <!-- The Ontology itself -->

  <owl:Ontology rdf:about="&alt;">
    <rdfs:label>AltLaw.org Vocabulary [DRAFT]</rdfs:label>
    <vann:preferredNamespacePrefix>alt</vann:preferredNamespacePrefix>
    <rdfs:comment>
      An RDF vocabulary for Semantic Web applications using data
      provided by AltLaw.org.  Many classes and properties here are
      borrowed directly from Bibliontology, Dublin Core, and the draft
      OAI4Courts specification, with comments indicating how they are
      used by AltLaw.

      THIS VOCABULARY IS EXPERIMENTAL AND SUBJECT TO MAJOR CHANGES.

      The RDF/XML source of this vocabulary can be found at
      http://github.com/lawcommons/altlaw-vocab
    </rdfs:comment>
    <rdfs:seeAlso rdf:resource="&bibo;"/>
    <rdfs:seeAlso rdf:resource="&dcterms;"/>
    <rdfs:seeAlso rdf:resource="http://topics.law.cornell.edu/wiki/lexcraft/oai4courts_overview"/>
  </owl:Ontology>


  <!-- CLASSES -->

  <owl:Class rdf:about="&alt;Court">
    <rdfs:label>alt:Court</rdfs:label>
    <rdfs:comment>
      Any court.
    </rdfs:comment>
    <rdfs:seeAlso rdf:resource="http://altlaw.org/courts"/>
    <rdfs:subClassOf rdf:resource="&foaf;Organization"/>
    <rdfs:isDefinedBy rdf:resource="&alt;"/>
  </owl:Class>

  <owl:Class rdf:about="&alt;Judgment">
    <rdfs:label>alt:Judgment</rdfs:label>
    <rdfs:comment>
      A determination by a Court on matters put before it.

      A Judgment is an abstract concept, the written form of which is
      a bibo:LegalDecision.  However, not all court judgments are
      written down.
    </rdfs:comment>
    <rdfs:isDefinedBy rdf:resource="&alt;"/>
  </owl:Class>

  <owl:Class rdf:abouc="&bibo;LegalDecision">
    <rdfs:label>bibo:LegalDecision</rdfs:label>
    <rdfs:comment>
      A written document containing the authoratitive judgment of a
      court.
    </rdfs:comment>
    <rdfs:isDefinedBy rdf:resource="&bibo;"/>
  </owl:Class>

  <owl:Class rdf:about="&alt;Opinion">
    <rdfs:label>alt:Opinion</rdfs:label>
    <rdfs:comment>
      A single written screed within a bibo:LegalDecision.  Represents
      the view of one judge or an agreement among judges, such as a
      majority opinion, concurrence, or dissent.
    </rdfs:comment>
    <rdfs:subClassOf rdf:resource="&bibo;LegalCaseDocument"/>
    <rdfs:subClassOf>
      <owl:Restriction>
        <owl:allValuesFrom rdf:resource="&alt;Decision"/>
        <owl:onProperty rdf:resource="&dcterms;isPartOf"/>
      </owl:Restriction>
    </rdfs:subClassOf>
    <rdfs:isDefinedBy rdf:resource="&alt;"/>
  </owl:Class>

  <owl:Class rdf:about="&alt;BluebookCitation">
    <rdfs:label>alt:BluebookCitation</rdfs:label>
    <rdfs:comment>
      A citation to a document in the form described by "A Uniform
      System of Citation", a.k.a. the Bluebook, available at
      http://www.legalbluebook.com/

      A BluebookCitation is typically composed of a title, one or more
      BluebookLocators, and a year and court in parentheses. Instances
      of this class should have, at a minimum, an rdf:value property
      pointing to the full citation as a string.

      Individual components may be represented by the properties
      dcterms:title, dcterms:date, and bibo:court.
      Volume/reporter/page locators may be represented with
      dcterms:hasPart properties pointing to instances of
      BluebookLocator.
    </rdfs:comment>
    <rdfs:isDefinedBy rdf:resource="&alt;"/>
  </owl:Class>

  <owl:Class rdf:about="&alt;BluebookLocator">
    <rdfs:label>alt:BluebookLocator</rdfs:label>
    <rdfs:comment>
      A Bluebook locator has three parts, as in "[volume] [reporter]
      [page]", with an optional "pincite" giving the page at which a
      particular reference is found.  Instances of this class should
      have, at a minimum, an rdf:value property pointing to the
      locator as a string.  Individual components may be represented
      by the properties bibo:volume, bibo:startPage, and
      dcterms:isPartOf pointing to an instance of bibo:CourtReporter
      or some other collection class.  Pincites may be represented
      with the alt:atPage or alt:atParagraph properties.
    </rdfs:comment>
    <rdfs:isDefinedBy rdf:resource="&alt;"/>
  </owl:Class>

  <owl:Class rdf:about="&alt;Errata">
    <rdfs:label>alt:Errata</rdfs:label>
    <rdfs:comment>
      A document listing corrections, modifications, or additions to
      another document.  We would like to have this in a
      machine-readable form such as a diff, but courts do not publish
      that way.
    </rdfs:comment>
    <rdfs:subClassOf rdf:resource="&bibo;Document"/>
    <rdfs:isDefinedBy rdf:resource="&alt;"/>
  </owl:Class>


  <!-- PROPERTIES -->

  <!-- Title properties -->

  <owl:DatatypeProperty rdf:about="&alt;fullTitle">
    <rdfs:label>alt:fullTitle</rdfs:label>
    <rdfs:comment>
      The full, formal title of the case, e.g. "Oliver Brown et
      al. v. Board of Education of Topeka et al."  A case should have
      only one full title.  Use "dcterms:title" if uncertain.
    </rdfs:comment>
    <rdfs:domain rdf:resource="&bibo;Document"/>
    <rdfs:subPropertyOf rdf:resource="&dcterms;title"/>
    <rdfs:isDefinedBy rdf:resource="&alt;"/>
  </owl:DatatypeProperty>

  <owl:DatatypeProperty rdf:about="&bibo;shortTitle">
    <rdfs:label>bibo:shortTitle</rdfs:label>
    <rdfs:comment>
      A shortened title of a case, as commonly used when citing or
      discussing the case, e.g. "Brown v. Board of Education" or just
      "Brown".  A case may have multiple short titles.  Use
      "dcterms:title" if uncertain.
    </rdfs:comment>
    <rdfs:isDefinedBy rdf:resource="&bibo;"/>
  </owl:DatatypeProperty>

  <owl:DatatypeProperty rdf:about="&dcterms;issued">
    <rdfs:label>dcterms:title</rdfs:label>
    <rdfs:comment>
      The title of a case.  This property is used when it is not clear
      if the value represents the full title or a short title.
    </rdfs:comment>
    <rdfs:seeAlso rdf:resource="&dcdoc;"/>
    <rdfs:isDefinedBy rdf:resource="&dcterms;"/>
    <rdfs:subPropertyOf rdf:resource="&dc;title"/>
  </owl:DatatypeProperty>


  <!-- Date properties -->

  <owl:DatatypeProperty rdf:about="&dcterms;date">
    <rdfs:label>dcterms:date</rdfs:label>
    <rdfs:comment>
      The date of a decision, vaguely assumed to be the date it was
      decided.  This may be the date "decided", "submitted", "issued",
      etc.  Datatype should be "xsd:date".
    </rdfs:comment>
    <rdfs:seeAlso rdf:resource="&dcdoc;"/>
    <rdfs:isDefinedBy rdf:resource="&dcterms;"/>
    <rdfs:subPropertyOf rdf:resource="&dc;date"/>
  </owl:DatatypeProperty>

  <owl:DatatypeProperty rdf:about="&dcterms;issued">
    <rdfs:label>dcterms:issued</rdfs:label>
    <rdfs:comment>
      The date a decision was published.  Use this property only when
      the date of publication is different from the date "decided".
    </rdfs:comment>
    <rdfs:seeAlso rdf:resource="&dcdoc;"/>
    <rdfs:isDefinedBy rdf:resource="&dcterms;"/>
    <rdfs:subPropertyOf rdf:resource="&dcterms;date"/>
  </owl:DatatypeProperty>


  <!-- Citation properties -->

  <owl:DatatypeProperty rdf:about="&alt;documentNumber">
    <rdfs:label>alt:documentNumber</rdfs:label>
    <rdfs:comment>
      The court-assigned document number within a docket.
    </rdfs:comment>
    <rdfs:subPropertyOf rdf:resource="&dcterms;identifier"/>
    <rdfs:domain rdf:resource="&bibo;LegalCaseDocument"/>
    <rdfs:range rdf:resource="&xsd;string"/>
    <rdfs:isDefinedBy rdf:resource="&alt;"/>
  </owl:DatatypeProperty>

  <owl:DatatypeProperty rdf:about="&alt;precedential">
    <rdfs:label>alt:precedential</rdfs:label>
    <rdfs:comment>
      Boolean indicating whether or not a decision is considered
      "precedential" (or, equivalently, "published") by the court that
      issued it.
    </rdfs:comment>
    <rdfs:domain rdf:resource="&bibo;LegalDecision"/>
    <rdfs:range rdf:resource="&xsd;boolean"/>
    <rdfs:isDefinedBy rdf:resource="&alt;"/>
  </owl:DatatypeProperty>



  <!-- File properties -->

  <owl:ObjectProperty rdf:about="&dcterms;hasFormat">
    <rdfs:label>dcterms:hasFormat</rdfs:label>
    <rdfs:comment>
      Link to another resource containing the same document in a
      different format.  The target will have an nie:mimeType
      property giving its MIME type.
    </rdfs:comment>
    <rdfs:seeAlso rdf:resource="&dcdoc;"/>
    <rdfs:isDefinedBy rdf:resource="&dcterms;"/>
    <rdfs:subPropertyOf rdf:resource="&dcterms;relation"/>
  </owl:ObjectProperty>

  <owl:ObjectProperty rdf:about="&nie;mimeType">
    <rdfs:label>nie:mimeType</rdfs:label>
    <rdfs:comment>
      The MIME type of a resource, from the list published by the
      IANA.
    </rdfs:comment>
    <rdfs:isDefinedBy rdf:resource="&nie;"/>
  </owl:ObjectProperty>


  <!-- Description properties -->

  <owl:DatatypeProperty rdf:about="&dcterms;abstract">
    <rdfs:label>dcterms:abstract</rdfs:label>
    <rdfs:comment>
      An abstract or summary of a decision.  Provided by some court
      web sites, but not considered part of the official decision.
    </rdfs:comment>
    <rdfs:seeAlso rdf:resource="&dcdoc;"/>
    <rdfs:isDefinedBy rdf:resource="&dcterms;"/>
    <rdfs:subPropertyOf rdf:resource="&dcterms;description"/>
  </owl:DatatypeProperty>

  <owl:DatatypeProperty rdf:about="&dcterms;subject">
    <rdfs:label>dcterms:subject</rdfs:label>
    <rdfs:comment>
      A keyword or broad topic heading for the case, such as
      "criminal" or "immigration".  Provided by some court web sites,
      but not considered part of the official decision.
    </rdfs:comment>
    <rdfs:seeAlso rdf:resource="&dcdoc;"/>
    <rdfs:isDefinedBy rdf:resource="&dcterms;"/>
    <rdfs:subPropertyOf rdf:resource="&dc;subject"/>
  </owl:DatatypeProperty>

  <owl:DatatypeProperty rdf:about="&dcterms;issued">
    <rdfs:label>dcterms:description</rdfs:label>
    <rdfs:comment>
      Free-text field to store any additional metadata about a case.
      This is where metadata scrapers put any information that they do
      not know how to parse.

      If a scraper knows something about the kind of data the field
      contains, it may prefix the contents with an identifier in ALL
      CAPS, such as "APPEAL FROM" or "HEARD BY".
    </rdfs:comment>
    <rdfs:seeAlso rdf:resource="&dcdoc;"/>
    <rdfs:isDefinedBy rdf:resource="&dcterms;"/>
    <rdfs:subPropertyOf rdf:resource="&dc;description"/>
  </owl:DatatypeProperty>

</rdf:RDF>
