<?xml version="1.0" encoding="UTF-8"?>
<rdf:RDF 
   xmlns:alt="http://id.altlaw.org/terms/"
   xmlns:bibo="http://purl.org/ontology/bibo/"
   xmlns:dcterms="http://purl.org/dc/terms/"
   xmlns:foaf="http://xmlns.com/foaf/0.1/"
   xmlns:owl="http://www.w3.org/2002/07/owl#"
   xmlns:rdf="http://www.w3.org/1999/02/22-rdf-syntax-ns#"
   xmlns:rdfs="http://www.w3.org/2000/01/rdf-schema#"
   xmlns:xsd="http://www.w3.org/2001/XMLSchema#">


  <!-- The Ontology itself -->

  <owl:Ontology rdf:about="http://id.altlaw.org/terms/">
    <rdfs:label>AltLaw.org Vocabulary [DRAFT]</rdfs:label>
    <rdfs:comment>
      An RDF vocabulary for Semantic Web applications using data
      provided by AltLaw.org.  The classes and properties defined here
      are intended to supplement and be used alongside other metadata
      vocabularies such as Dublin Core (http://purl.org/dc/terms/) and
      Bibliontology (http://purl.org/ontology/bibo/).

      This vocabulary borrows some definitions from the OAI4Courts draft
      specification at
      http://topics.law.cornell.edu/wiki/lexcraft/oai4courts_overview

      This vocabulary redefines some terms that exist in other
      ontologies but are considered "unstable"
      (e.g. "bibo:LegalDecision").

      THIS VOCABULARY IS EXPERIMENTAL AND SUBJECT TO MAJOR CHANGES.

      The RDF/XML source of this vocabulary can be found at
      http://github.com/lawcommons/altlaw-vocab/tree/master/altlaw-vocab-1.rdf
    </rdfs:comment>
  </owl:Ontology>


  <!-- CLASSES -->

  <owl:Class rdf:about="http://id.altlaw.org/terms/Court">
    <rdfs:label>Court</rdfs:label>
    <rdfs:comment>
      Any court.
    </rdfs:comment>
    <rdfs:seeAlso rdf:resource="http://altlaw.org/courts"/>
    <rdfs:subClassOf rdf:resource="http://xmlns.com/foaf/0.1/Organization"/>
    <rdfs:isDefinedBy rdf:resource="http://id.altlaw.org/terms/"/>
  </owl:Class>

  <owl:Class rdf:about="http://id.altlaw.org/terms/Case">
    <rdfs:label>Case</rdfs:label>
    <rdfs:comment>
      A single dispute among two or more parties.  It may be argued in
      multiple Courts at different times, and may result in multiple
      Judgments.
    </rdfs:comment>
    <rdfs:isDefinedBy rdf:resource="http://id.altlaw.org/terms/"/>
  </owl:Class>

  <owl:Class rdf:about="http://id.altlaw.org/terms/Judgment">
    <rdfs:label>Judgment</rdfs:label>
    <rdfs:comment>
      A determination by a Court on matters put before it.

      A Judgment is an abstract concept, which takes its written form
      in a Decision.  However, Judgments may exist that have no
      written Decisions.  A Judgment may dispose of multiple Cases.
    </rdfs:comment>
    <rdfs:isDefinedBy rdf:resource="http://id.altlaw.org/terms/"/>
  </owl:Class>

  <owl:Class rdf:about="http://id.altlaw.org/terms/Decision">
    <rdfs:label>Decision</rdfs:label>
    <rdfs:comment>
      The written form of a Judgment.  A decision may be a complete
      document in and of itself, or it contain multiple Opinions with
      "dcterms:hasPart".
    </rdfs:comment>
    <owl:sameAs rdf:resource="http://purl.org/ontology/bibo/LegalDecision"/>
    <rdfs:subClassOf rdf:resource="http://purl.org/ontology/bibo/LegalCaseDocument"/>
    <rdfs:seeAlso rdf:resource="http://bibliontology.com/"/>
    <rdfs:isDefinedBy rdf:resource="http://id.altlaw.org/terms/"/>
  </owl:Class>

  <owl:Class rdf:about="http://id.altlaw.org/terms/Opinion">
    <rdfs:label>Opinion</rdfs:label>
    <rdfs:comment>
      A single written screed within a Decision.  Represents the view
      of one judge or an agreement among judges, such as a majority
      opinion, concurrence, or dissent.
    </rdfs:comment>
    <rdfs:subClassOf rdf:resource="http://purl.org/ontology/bibo/LegalCaseDocument"/>
    <rdfs:isDefinedBy rdf:resource="http://id.altlaw.org/terms/"/>
  </owl:Class>

  <owl:Class rdf:about="http://id.altlaw.org/terms/Errata">
    <rdfs:label>Errata</rdfs:label>
    <rdfs:comment>
      A document listing corrections, modifications, or additions to
      another document.  We would like to have this in a
      machine-readable form such as a diff, but courts do not publish
      that way.
    </rdfs:comment>
    <rdfs:subClassOf rdf:resource="http://purl.org/ontology/bibo/Document"/>
    <rdfs:isDefinedBy rdf:resource="http://id.altlaw.org/terms/"/>
  </owl:Class>

  <owl:Class rdf:about="http://id.altlaw.org/terms/Process">
    <rdfs:label>Process</rdfs:label>
    <rdfs:comment>
      A single execution of an automated operation.
    </rdfs:comment>
    <rdfs:isDefinedBy rdf:resource="http://id.altlaw.org/terms/"/>
  </owl:Class>

  <owl:Class rdf:about="http://id.altlaw.org/terms/Crawl">
    <rdfs:label>Crawl</rdfs:label>
    <rdfs:comment>
      A Crawl is a single run of an automated process that retrieves
      and processes Internet resources.
    </rdfs:comment>
    <rdfs:subClassOf rdf:resource="http://id.altlaw.org/terms/Process"/>
    <rdfs:isDefinedBy rdf:resource="http://id.altlaw.org/terms/"/>
  </owl:Class>

  <owl:Class rdf:about="http://id.altlaw.org/terms/File">
    <rdfs:label>File</rdfs:label>
    <rdfs:comment>
      A concrete digital representation of a document.  As opposed to
      the abstract concept of a document and the facts it embodies, a
      File is a finite sequence of bytes in a particular format and/or
      encoding.  OAI4Courts calls this a "writing".
    </rdfs:comment>
    <rdfs:isDefinedBy rdf:resource="http://id.altlaw.org/terms/"/>
  </owl:Class>

  <owl:Class rdf:about="http://id.altlaw.org/terms/Download">
    <rdfs:label>Download</rdfs:label>
    <rdfs:comment>
      Record of downloading a file from an Internet resource.  Used
      for logging HTTP requests/responses.
    </rdfs:comment>
    <rdfs:subClassOf rdf:resource="http://id.altlaw.org/terms/Process"/>
    <rdfs:isDefinedBy rdf:resource="http://id.altlaw.org/terms/"/>
  </owl:Class>


  <!-- PROPERTIES -->

  <rdfs:Property rdf:about="http://id.altlaw.org/terms/court">
    <rdfs:label>court</rdfs:label>
    <rdfs:comment>
      The court which originated a Judgment.
    </rdfs:comment>
    <rdfs:subPropertyOf rdf:resource="http://purl.org/dc/terms/coverage"/>
    <rdfs:domain rdf:resource="http://id.altlaw.org/terms/Judgment"/>
    <rdfs:range rdf:resource="http://id.altlaw.org/terms/Court"/>
    <owl:sameAs rdf:resource="http://purl.org/ontology/bibo/court"/>
    <rdfs:isDefinedBy rdf:resource="http://id.altlaw.org/terms/"/>
  </rdfs:Property>
  
  <rdfs:Property rdf:about="http://id.altlaw.org/terms/docketNumber">
    <rdfs:label>docketNumber</rdfs:label>
    <rdfs:comment>
      The docket number associated with a Document or Case.

      A single case may have multiple docket numbers attached to it.
      The range of this property is any string, which may include
      punctuation such as hyphens, but it should be a single docket
      number rather than a series such as "10-102; 10-103".  The
      string also should not contain abbreviations for "Number" such
      as "No." or "Nos.".
    </rdfs:comment>
    <rdfs:subPropertyOf rdf:resource="http://purl.org/dc/terms/identifier"/>
    <rdfs:range rdf:resource="http://www.w3.org/2001/XMLSchema#string"/>
    <rdfs:isDefinedBy rdf:resource="http://id.altlaw.org/terms/"/>
  </rdfs:Property>

  <rdfs:Property rdf:about="http://id.altlaw.org/terms/bluebookIdentifier">
    <rdfs:label>bluebookIdentifier</rdfs:label>
    <rdfs:comment>
      A citation to a decision in the form described by "A Uniform
      System of Citation", a.k.a. the Bluebook, available at
      http://www.legalbluebook.com/

      Values of this property should use the three-part syntax
      "[volume] [reporter] [page]".  Additional information such as
      title, date, court, and pinpoint citations ("pincites") should
      be omitted.  Section numbers may be used instead of pages, as in
      "17 U.S.C. &#167; 705".

      A single value of this property must not include parallel
      citations, but a single decision may have multiple
      bluebookIdentifiers, one for each parallel citation.
    </rdfs:comment>
    <rdfs:subPropertyOf rdf:resource="http://purl.org/dc/terms/identifier"/>
    <rdfs:domain rdf:resource="http://id.altlaw.org/terms/Decision"/>
    <rdfs:range rdf:resource="http://www.w3.org/2001/XMLSchema#string"/>
    <rdfs:isDefinedBy rdf:resource="http://id.altlaw.org/terms/"/>
  </rdfs:Property>

  <rdfs:Property rdf:about="http://id.altlaw.org/terms/precedential">
    <rdfs:label>precedential</rdfs:label>
    <rdfs:comment>
      Boolean indicating whether or not a decision is considered
      "precedential" (or, equivalently, "published") by the court
      that issued it.
    </rdfs:comment>
    <rdfs:domain rdf:resource="http://id.altlaw.org/terms/Judgment"/>
    <rdfs:range rdf:resource="http://www.w3.org/2001/XMLSchema#boolean"/>
    <rdfs:isDefinedBy rdf:resource="http://id.altlaw.org/terms/"/>
  </rdfs:Property>

  <rdfs:Property rdf:about="http://id.altlaw.org/terms/decided">
    <rdfs:label>decided</rdfs:label>
    <rdfs:comment>
      Date that a court decision/ruling/order was decided.  May or may
      not be the same as date of publication ("dcterms:issued").  This
      is the preferred date to use when describing a court decision.
    </rdfs:comment>
    <rdfs:subPropertOf rdf:resource="http://purl.org/dc/terms/date"/>
    <rdfs:domain rdf:resource="http://id.altlaw.org/terms/Judgment"/>
    <rdfs:range rdf:resource="http://www.w3.org/2001/XMLSchema#date"/>
    <rdfs:isDefinedBy rdf:resource="http://id.altlaw.org/terms/"/>
  </rdfs:Property>

  <rdfs:Property rdf:about="http://id.altlaw.org/terms/argued">
    <rdfs:label>argued</rdfs:label>
    <rdfs:comment>
      Date that a case was argued before a court.  A case may have
      many dates of argument.
    </rdfs:comment>
    <rdfs:subPropertOf rdf:resource="http://purl.org/dc/terms/date"/>
    <rdfs:range rdf:resource="http://www.w3.org/2001/XMLSchema#date"/>
    <owl:sameAs rdf:resource="http://purl.org/ontology/bibo/argued"/>
    <rdfs:isDefinedBy rdf:resource="http://id.altlaw.org/terms/"/>
  </rdfs:Property>

  <rdfs:Property rdf:about="http://id.altlaw.org/terms/amends">
    <rdfs:label>amends</rdfs:label>
    <rdfs:comment>
      Link between an Errata document and the Document it
      modifies/corrects.
    </rdfs:comment>
    <rdfs:domain rdf:resource="http://id.altlaw.org/terms/Errata"/>
    <rdfs:range rdf:resource="http://purl.org/ontology/bibo/Document"/>
    <rdfs:isDefinedBy rdf:resource="http://id.altlaw.org/terms/"/>
  </rdfs:Property>

  <rdfs:Property rdf:about="http://id.altlaw.org/terms/mimeType">
    <rdfs:label>mimeType</rdfs:label>
    <rdfs:comment>
      The MIME type of a File, a literal string such as "application/pdf".

      This property is included to avoid potential confusion over the
      correct usage of "dcterms:format", which has a non-literal
      range.
    </rdfs:comment>
    <rdfs:seeAlso rdf:resource="http://www.iana.org/assignments/media-types/"/>
    <rdfs:domain rdf:resource="http://id.altlaw.org/terms/File"/>
    <rdfs:range rdf:resource="http://www.w3.org/2001/XMLSchema#string"/>
    <rdfs:subPropertyOf rdf:resource="http://purl.org/dc/elements/1.1/format"/>
    <rdfs:isDefinedBy rdf:resource="http://id.altlaw.org/terms/"/>
  </rdfs:Property>

  <rdfs:Property rdf:about="http://id.altlaw.org/terms/charset">
    <rdfs:label>charset</rdfs:label>
    <rdfs:comment>
      The binary character encoding used by a File.  The value of this
      property should be a literal string taken from the list at
      iana.org.

      When a character set has multiple names, the name given as the
      "preferred MIME name" by iana.org should be used.  Preferred
      names for common character sets are "US-ASCII", "ISO-8859-1",
      "windows-1252", and "UTF-8".
    </rdfs:comment>
    <rdfs:seeAlso rdf:resource="http://www.iana.org/assignments/character-sets"/>
    <rdfs:domain rdf:resource="http://id.altlaw.org/terms/File"/>
    <rdfs:range rdf:resource="http://www.w3.org/2001/XMLSchema#string"/>
    <rdfs:subPropertyOf rdf:resource="http://purl.org/dc/elements/1.1/format"/>
    <rdfs:isDefinedBy rdf:resource="http://id.altlaw.org/terms/"/>
  </rdfs:Property>

  <rdfs:Property rdf:about="http://id.altlaw.org/terms/started">
    <rdfs:label>started</rdfs:label>
    <rdfs:comment>
      Timestamp when a process began.
    </rdfs:comment>
    <rdfs:subPropertyOf rdf:resource="http://purl.org/dc/terms/created"/>
    <rdfs:domain rdf:resource="http://id.altlaw.org/terms/Process"/>
    <rdfs:range rdf:resource="http://www.w3.org/2001/XMLSchema#dateTime"/>
    <rdfs:isDefinedBy rdf:resource="http://id.altlaw.org/terms/"/>
  </rdfs:Property>

  <rdfs:Property rdf:about="http://id.altlaw.org/terms/finished">
    <rdfs:label>finished</rdfs:label>
    <rdfs:comment>
      Timestamp when a process was completed.
    </rdfs:comment>
    <rdfs:subPropertyOf rdf:resource="http://purl.org/dc/terms/date"/>
    <rdfs:domain rdf:resource="http://id.altlaw.org/terms/Process"/>
    <rdfs:range rdf:resource="http://www.w3.org/2001/XMLSchema#dateTime"/>
    <rdfs:isDefinedBy rdf:resource="http://id.altlaw.org/terms/"/>
  </rdfs:Property>

  <rdfs:Property rdf:about="http://id.altlaw.org/terms/discovered">
    <rdfs:label>discovered</rdfs:label>
    <rdfs:comment>
      The "discovered" property links a Crawl to the entities that it
      finds.
    </rdfs:comment>
    <rdfs:isDefinedBy rdf:resource="http://id.altlaw.org/terms/"/>
    <rdfs:domain rdf:resource="http://id.altlaw.org/terms/Crawl"/>
  </rdfs:Property>

  <rdfs:Property rdf:about="http://id.altlaw.org/terms/downloaded">
    <rdfs:label>downloaded</rdfs:label>
    <rdfs:comment>
      A single Download performed during a Crawl.
    </rdfs:comment>
    <rdfs:isDefinedBy rdf:resource="http://id.altlaw.org/terms/"/>
    <rdfs:domain rdf:resource="http://id.altlaw.org/terms/Crawl"/>
    <rdfs:range rdf:resource="http://id.altlaw.org/terms/Download"/>
  </rdfs:Property>

  <rdfs:Property rdf:about="http://id.altlaw.org/terms/url">
    <rdfs:label>url</rdfs:label>
    <rdfs:comment>
      The URL from which a Download was retrieved.
    </rdfs:comment>
    <rdfs:isDefinedBy rdf:resource="http://id.altlaw.org/terms/"/>
    <rdfs:domain rdf:resource="http://id.altlaw.org/terms/Download"/>
    <rdfs:range rdf:resource="http://www.w3.org/2001/XMLSchema#string"/>
  </rdfs:Property>

  <rdfs:Property rdf:about="http://id.altlaw.org/terms/httpRequest">
    <rdfs:label>httpRequest</rdfs:label>
    <rdfs:comment>
      A complete log of the HTTP request sent to a remote server,
      containing both HTTP headers and entity body.
    </rdfs:comment>
    <rdfs:isDefinedBy rdf:resource="http://id.altlaw.org/terms/"/>
    <rdfs:domain rdf:resource="http://id.altlaw.org/terms/Download"/>
    <rdfs:range rdf:resource="http://www.w3.org/2001/XMLSchema#string"/>
  </rdfs:Property>

  <rdfs:Property rdf:about="http://id.altlaw.org/terms/httpResponse">
    <rdfs:label>httpResponse</rdfs:label>
    <rdfs:comment>
      A complete log of the HTTP response received from a remote
      server, containing both HTTP headers and entity body.
    </rdfs:comment>
    <rdfs:isDefinedBy rdf:resource="http://id.altlaw.org/terms/"/>
    <rdfs:domain rdf:resource="http://id.altlaw.org/terms/Download"/>
    <rdfs:range rdf:resource="http://www.w3.org/2001/XMLSchema#string"/>
  </rdfs:Property>

  <!-- PROPERTIES DEFINED IN OTHER ONTOLOGIES -->

  <rdfs:Property rdf:about="http://purl.org/dc/terms/date">
    <rdfs:label>dcterms:date</rdfs:label>
    <rdfs:comment>
      The date of a decision.  Use this property only when more
      specific dates, such as "decided" or "issued", are unknown.
      Datatype should be "xsd:date".
    </rdfs:comment>
    <rdfs:seeAlso rdf:resource="http://dublincore.org/documents/dcmi-terms/"/>
    <rdfs:isDefinedBy rdf:resource="http://purl.org/dc/terms/"/>
    <rdfs:subPropertyOf rdf:resource="http://purl.org/dc/elements/1.1/date"/>
  </rdfs:Property>

  <rdfs:Property rdf:about="http://purl.org/dc/terms/issued">
    <rdfs:label>dcterms:issued</rdfs:label>
    <rdfs:comment>
      The date a Judgment was published.  Use this property only when
      the date of publication is different from the date "decided".
    </rdfs:comment>
    <rdfs:seeAlso rdf:resource="http://dublincore.org/documents/dcmi-terms/"/>
    <rdfs:isDefinedBy rdf:resource="http://purl.org/dc/terms/"/>
    <rdfs:subPropertyOf rdf:resource="http://purl.org/dc/terms/date"/>
  </rdfs:Property>

  <rdfs:Property rdf:about="http://purl.org/dc/terms/issued">
    <rdfs:label>dcterms:title</rdfs:label>
    <rdfs:comment>
      The title of a case.  The value of this property should be the
      full, formal title of the case, e.g. "Oliver Brown et
      al. v. Board of Education of Topeka et al."  A case should have
      only one full title.
    </rdfs:comment>
    <rdfs:seeAlso rdf:resource="http://dublincore.org/documents/dcmi-terms/"/>
    <rdfs:isDefinedBy rdf:resource="http://purl.org/dc/terms/"/>
    <rdfs:subPropertyOf rdf:resource="http://purl.org/dc/elements/1.1/title"/>
  </rdfs:Property>

  <rdfs:Property rdf:about="http://purl.org/ontology/bibo/shortTitle">
    <rdfs:label>bibo:shortTitle</rdfs:label>
    <rdfs:comment>
      A shortened title of a case, as commonly used when citing or
      discussing the case, e.g. "Brown v. Board of Education" or just
      "Brown".  A case may have multiple short titles.
    </rdfs:comment>
    <rdfs:isDefinedBy rdf:resource="http://purl.org/ontology/bibo/"/>
    <rdfs:seeAlso rdf:resource="http://bibliontology.com/"/>
    <rdfs:subPropertyOf rdf:resource="http://purl.org/dc/terms/alternative"/>
  </rdfs:Property>

  <rdfs:Property rdf:about="http://purl.org/dc/terms/hasFormat">
    <rdfs:label>dcterms:hasFormat</rdfs:label>
    <rdfs:comment>
      Link from an abstract entity, such as a Decision, to its
      concrete representation, such as a File.
    </rdfs:comment>
    <rdfs:seeAlso rdf:resource="http://dublincore.org/documents/dcmi-terms/"/>
    <rdfs:isDefinedBy rdf:resource="http://purl.org/dc/terms/"/>
    <rdfs:subPropertyOf rdf:resource="http://purl.org/dc/terms/relation"/>
  </rdfs:Property>

  <rdfs:Property rdf:about="http://purl.org/dc/terms/abstract">
    <rdfs:label>dcterms:abstract</rdfs:label>
    <rdfs:comment>
      An abstract or summary of a decision.  Provided by some court
      web sites, but not considered part of the official decision.
    </rdfs:comment>
    <rdfs:seeAlso rdf:resource="http://dublincore.org/documents/dcmi-terms/"/>
    <rdfs:isDefinedBy rdf:resource="http://purl.org/dc/terms/"/>
    <rdfs:subPropertyOf rdf:resource="http://purl.org/dc/terms/description"/>
  </rdfs:Property>

  <rdfs:Property rdf:about="http://purl.org/dc/terms/subject">
    <rdfs:label>dcterms:subject</rdfs:label>
    <rdfs:comment>
      A keyword or broad topic heading for the case, such as
      "criminal" or "immigration".  Provided by some court web sites,
      but not considered part of the official decision.
    </rdfs:comment>
    <rdfs:seeAlso rdf:resource="http://dublincore.org/documents/dcmi-terms/"/>
    <rdfs:isDefinedBy rdf:resource="http://purl.org/dc/terms/"/>
    <rdfs:subPropertyOf rdf:resource="http://purl.org/dc/elements/1.1/subject"/>
  </rdfs:Property>

  <rdfs:Property rdf:about="http://purl.org/dc/terms/issued">
    <rdfs:label>dcterms:description</rdfs:label>
    <rdfs:comment>
      Free-text field to store any additional metadata about a case.
      This is where metadata scrapers put any information that they do
      not know how to parse.

      If a scraper knows something about the kind of data the field
      contains, it may prefix the contents with an identifier in ALL
      CAPS, such as "APPEAL FROM" or "HEARD BY".
    </rdfs:comment>
    <rdfs:seeAlso rdf:resource="http://dublincore.org/documents/dcmi-terms/"/>
    <rdfs:isDefinedBy rdf:resource="http://purl.org/dc/terms/"/>
    <rdfs:subPropertyOf rdf:resource="http://purl.org/dc/elements/1.1/description"/>
  </rdfs:Property>

</rdf:RDF>
