<?xml version="1.0"?>


<!DOCTYPE rdf:RDF [
    <!ENTITY vocab "http://id.altlaw.org/vocab/" >
    <!ENTITY vann "http://purl.org/vocab/vann/" >
    <!ENTITY owl "http://www.w3.org/2002/07/owl#" >
    <!ENTITY xsd "http://www.w3.org/2001/XMLSchema#" >
    <!ENTITY owl2xml "http://www.w3.org/2006/12/owl2-xml#" >
    <!ENTITY rdfs "http://www.w3.org/2000/01/rdf-schema#" >
    <!ENTITY rdf "http://www.w3.org/1999/02/22-rdf-syntax-ns#" >
]>


<rdf:RDF xmlns="http://id.altlaw.org/vocab/"
     xml:base="http://id.altlaw.org/vocab/"
     xmlns:rdfs="http://www.w3.org/2000/01/rdf-schema#"
     xmlns:owl2xml="http://www.w3.org/2006/12/owl2-xml#"
     xmlns:owl="http://www.w3.org/2002/07/owl#"
     xmlns:xsd="http://www.w3.org/2001/XMLSchema#"
     xmlns:rdf="http://www.w3.org/1999/02/22-rdf-syntax-ns#"
     xmlns:vann="http://purl.org/vocab/vann/"
     xmlns:vocab="http://id.altlaw.org/vocab/">
    <owl:Ontology rdf:about="">
        <rdfs:label xml:lang="en"
            >AltLaw Vocabulary</rdfs:label>
        <rdfs:comment xml:lang="en"
            >Vocabulary for describing legal references collected and maintained by AltLaw.org.</rdfs:comment>
        <vann:preferredNamespacePrefix>alt</vann:preferredNamespacePrefix>
        <owl:versionInfo
            >http://id.altlaw.org/vocab/1.0/</owl:versionInfo>
    </owl:Ontology>
    


    <!-- 
    ///////////////////////////////////////////////////////////////////////////////////////
    //
    // Annotation properties
    //
    ///////////////////////////////////////////////////////////////////////////////////////
     -->

    <owl:AnnotationProperty rdf:about="&vann;preferredNamespacePrefix"/>
    


    <!-- 
    ///////////////////////////////////////////////////////////////////////////////////////
    //
    // Object Properties
    //
    ///////////////////////////////////////////////////////////////////////////////////////
     -->

    


    <!-- http://id.altlaw.org/vocab/court -->

    <owl:ObjectProperty rdf:about="court">
        <rdfs:label xml:lang="en">court</rdfs:label>
        <rdfs:comment xml:lang="en"
            >Court which produces a document or to which a document was submitted.</rdfs:comment>
        <rdfs:range rdf:resource="Court"/>
        <rdfs:domain rdf:resource="Document"/>
    </owl:ObjectProperty>
    


    <!-- http://id.altlaw.org/vocab/errata -->

    <owl:ObjectProperty rdf:about="errata">
        <rdfs:label xml:lang="en">errata</rdfs:label>
        <rdfs:comment xml:lang="en"
            >Link from a Document to an Errata document that corrects or modifies it.</rdfs:comment>
        <rdfs:domain rdf:resource="Document"/>
        <rdfs:range rdf:resource="Errata"/>
    </owl:ObjectProperty>
    


    <!-- http://id.altlaw.org/vocab/incite -->

    <owl:ObjectProperty rdf:about="incite">
        <rdfs:label xml:lang="en"
            >incoming citation</rdfs:label>
        <rdfs:comment xml:lang="en"
            >Incoming citation; i.e., a citation TO this document FROM some other document.</rdfs:comment>
        <rdfs:domain rdf:resource="Document"/>
        <rdfs:range rdf:resource="Document"/>
    </owl:ObjectProperty>
    


    <!-- http://id.altlaw.org/vocab/outcite -->

    <owl:ObjectProperty rdf:about="outcite">
        <rdfs:label xml:lang="en"
            >outgoing citation</rdfs:label>
        <rdfs:comment xml:lang="en"
            >Outgoing citation; i.e., a citation FROM this document TO some other document.</rdfs:comment>
        <rdfs:domain rdf:resource="Document"/>
        <rdfs:range rdf:resource="Document"/>
    </owl:ObjectProperty>
    


    <!-- http://id.altlaw.org/vocab/representation -->

    <owl:ObjectProperty rdf:about="representation">
        <rdfs:label xml:lang="en">representation</rdfs:label>
        <rdfs:comment xml:lang="en"
            >Link from a document to one of its concrete representations.</rdfs:comment>
        <rdfs:domain rdf:resource="Document"/>
        <rdfs:range rdf:resource="File"/>
    </owl:ObjectProperty>
    


    <!-- 
    ///////////////////////////////////////////////////////////////////////////////////////
    //
    // Data properties
    //
    ///////////////////////////////////////////////////////////////////////////////////////
     -->

    


    <!-- http://id.altlaw.org/vocab/bluebookLocator -->

    <owl:DatatypeProperty rdf:about="bluebookLocator">
        <rdfs:label xml:lang="en"
            >Bluebook locator</rdfs:label>
        <rdfs:comment xml:lang="en"
            >Citation form, following Bluebook conventions, containing only the minimum necessary information to identify a document, usually given as &quot;[volume] [reporter] [page]&quot; with an optional pincite.</rdfs:comment>
        <rdfs:domain rdf:resource="Document"/>
    </owl:DatatypeProperty>
    


    <!-- http://id.altlaw.org/vocab/caseNumber -->

    <owl:DatatypeProperty rdf:about="caseNumber">
        <rdfs:label xml:lang="en">case number</rdfs:label>
        <rdfs:comment xml:lang="en"
            >A single, court-assigned case number.  Usually, this is the same as the docket number, and the docketNumber property is preferred.  A few courts distinguish between &quot;case numbers&quot; and &quot;docket numbers&quot; however, and this property should be used then.</rdfs:comment>
        <rdfs:domain rdf:resource="Document"/>
    </owl:DatatypeProperty>
    


    <!-- http://id.altlaw.org/vocab/dateDecided -->

    <owl:DatatypeProperty rdf:about="dateDecided">
        <rdfs:label xml:lang="en">date decided</rdfs:label>
        <rdfs:comment xml:lang="en"
            >The date a court decision was decided.  Often, but not always, the same as the publication date.</rdfs:comment>
        <rdfs:domain rdf:resource="Document"/>
        <rdfs:range rdf:resource="&xsd;date"/>
    </owl:DatatypeProperty>
    


    <!-- http://id.altlaw.org/vocab/datePublished -->

    <owl:DatatypeProperty rdf:about="datePublished">
        <rdfs:label xml:lang="en">date published</rdfs:label>
        <rdfs:comment xml:lang="en"
            >Date a document was published.</rdfs:comment>
        <rdfs:domain rdf:resource="Document"/>
        <rdfs:range rdf:resource="&xsd;date"/>
    </owl:DatatypeProperty>
    


    <!-- http://id.altlaw.org/vocab/docid -->

    <owl:DatatypeProperty rdf:about="docid">
        <rdf:type rdf:resource="&owl;FunctionalProperty"/>
        <rdfs:label xml:lang="en">document ID</rdfs:label>
        <rdfs:comment xml:lang="en"
            >Document ID, an integer uniquely identifying the document within AltLaw&#39;s database.</rdfs:comment>
        <rdfs:domain rdf:resource="Document"/>
        <rdfs:range rdf:resource="&xsd;integer"/>
    </owl:DatatypeProperty>
    


    <!-- http://id.altlaw.org/vocab/docketNumber -->

    <owl:DatatypeProperty rdf:about="docketNumber">
        <rdfs:label xml:lang="en">docket number</rdfs:label>
        <rdfs:comment xml:lang="en"
            >A single, court-assigned docket number.</rdfs:comment>
        <rdfs:domain rdf:resource="Document"/>
    </owl:DatatypeProperty>
    


    <!-- http://id.altlaw.org/vocab/documentNumber -->

    <owl:DatatypeProperty rdf:about="documentNumber">
        <rdfs:label xml:lang="en">document number</rdfs:label>
        <rdfs:comment xml:lang="en"
            >A single, court-assigned number for one document within a collection of documents associated with a legal proceeding.</rdfs:comment>
        <rdfs:domain rdf:resource="Document"/>
    </owl:DatatypeProperty>
    


    <!-- http://id.altlaw.org/vocab/fullName -->

    <owl:DatatypeProperty rdf:about="fullName">
        <rdfs:label xml:lang="en">full name</rdfs:label>
        <rdfs:comment xml:lang="en"
            >Full-length, formal, official name of a court.</rdfs:comment>
        <rdfs:domain rdf:resource="Court"/>
    </owl:DatatypeProperty>
    


    <!-- http://id.altlaw.org/vocab/fullTitle -->

    <owl:DatatypeProperty rdf:about="fullTitle">
        <rdfs:label xml:lang="en">full title</rdfs:label>
        <rdfs:comment xml:lang="en"
            >The full-length title of a legal case, containing the full names of all parties, e.g., &quot;Oliver Brown et al. v. Board of Education of Topeka et al.&quot;  A case should have only one full title.</rdfs:comment>
        <rdfs:domain rdf:resource="Document"/>
    </owl:DatatypeProperty>
    


    <!-- http://id.altlaw.org/vocab/mimeType -->

    <owl:DatatypeProperty rdf:about="mimeType">
        <rdfs:label xml:lang="en">MIME type</rdfs:label>
        <rdfs:comment xml:lang="en"
            >Internet MIME type of a file.  May only include the &quot;major/minor&quot; string, with no additional attributes, such as &quot;charset.&quot;</rdfs:comment>
        <rdfs:domain rdf:resource="File"/>
    </owl:DatatypeProperty>
    


    <!-- http://id.altlaw.org/vocab/norobots -->

    <owl:DatatypeProperty rdf:about="norobots">
        <rdfs:label xml:lang="en"
            >no search engine robots</rdfs:label>
        <rdfs:comment xml:lang="en"
            >If true, the document should be blocked from search engine robots using META tags and/or robots.txt</rdfs:comment>
        <rdfs:domain rdf:resource="Document"/>
        <rdfs:range rdf:resource="&xsd;boolean"/>
    </owl:DatatypeProperty>
    


    <!-- http://id.altlaw.org/vocab/precedential -->

    <owl:DatatypeProperty rdf:about="precedential">
        <rdfs:label xml:lang="en">precedential?</rdfs:label>
        <rdfs:comment xml:lang="en"
            >True/false value; true if the document  is considered precedential, suitable for citation, or &quot;published&quot; by the court that issued it.</rdfs:comment>
        <rdfs:domain rdf:resource="Document"/>
        <rdfs:range rdf:resource="&xsd;boolean"/>
    </owl:DatatypeProperty>
    


    <!-- http://id.altlaw.org/vocab/removed -->

    <owl:DatatypeProperty rdf:about="removed">
        <rdfs:label xml:lang="en">removed</rdfs:label>
        <rdfs:comment xml:lang="en"
            >If true, the document has been removed from the database.</rdfs:comment>
        <rdfs:domain rdf:resource="Document"/>
        <rdfs:range rdf:resource="&xsd;boolean"/>
    </owl:DatatypeProperty>
    


    <!-- http://id.altlaw.org/vocab/shortName -->

    <owl:DatatypeProperty rdf:about="shortName">
        <rdfs:label xml:lang="en">short name</rdfs:label>
        <rdfs:comment xml:lang="en"
            >Shortened, but not fully abbreviated, name of a court.</rdfs:comment>
        <rdfs:domain rdf:resource="Court"/>
    </owl:DatatypeProperty>
    


    <!-- http://id.altlaw.org/vocab/shortTitle -->

    <owl:DatatypeProperty rdf:about="shortTitle">
        <rdfs:label xml:lang="en">short title</rdfs:label>
        <rdfs:comment xml:lang="en"
            >An abbreviated title of a case, as commonly used when citing or discussing the case.  Usually only includes the last name of each party, e.g. &quot;Brown v. Board of Education&quot; or just &quot;Brown&quot;.  A case may have multiple short titles.</rdfs:comment>
        <rdfs:domain rdf:resource="Document"/>
    </owl:DatatypeProperty>
    


    <!-- http://id.altlaw.org/vocab/sourceUrl -->

    <owl:DatatypeProperty rdf:about="sourceUrl">
        <rdfs:label xml:lang="en">source URL</rdfs:label>
        <rdfs:comment xml:lang="en"
            >URL from which a File was downloaded, or can be downloaded.</rdfs:comment>
        <rdfs:domain rdf:resource="File"/>
        <rdfs:range rdf:resource="&xsd;anyURI"/>
    </owl:DatatypeProperty>
    


    <!-- http://id.altlaw.org/vocab/textSize -->

    <owl:DatatypeProperty rdf:about="textSize">
        <rdfs:label xml:lang="en">text size</rdfs:label>
        <rdfs:comment xml:lang="en"
            >Number of characters in the plain-text representation of the document.</rdfs:comment>
        <rdfs:domain rdf:resource="Document"/>
        <rdfs:range rdf:resource="&xsd;integer"/>
    </owl:DatatypeProperty>
    


    <!-- http://id.altlaw.org/vocab/wikipediaName -->

    <owl:DatatypeProperty rdf:about="wikipediaName">
        <rdfs:label xml:lang="en">Wikipedia name</rdfs:label>
        <rdfs:comment xml:lang="en"
            >Name appearing in the URL of a Wikipedia page describing the resource.  Can be used to construct URLs for Wikipedia or DBpedia.</rdfs:comment>
        <rdfs:domain rdf:resource="Court"/>
    </owl:DatatypeProperty>
    


    <!-- 
    ///////////////////////////////////////////////////////////////////////////////////////
    //
    // Classes
    //
    ///////////////////////////////////////////////////////////////////////////////////////
     -->

    


    <!-- http://id.altlaw.org/vocab/Court -->

    <owl:Class rdf:about="Court">
        <rdfs:label xml:lang="en">Court</rdfs:label>
        <rdfs:comment xml:lang="en"
            >Any court which can render judgments.</rdfs:comment>
    </owl:Class>
    


    <!-- http://id.altlaw.org/vocab/Decision -->

    <owl:Class rdf:about="Decision">
        <rdfs:label xml:lang="en">Decision</rdfs:label>
        <rdfs:subClassOf rdf:resource="Document"/>
        <rdfs:comment xml:lang="en"
            >A written document containing the authoratitve judgment of a court.</rdfs:comment>
    </owl:Class>
    


    <!-- http://id.altlaw.org/vocab/Document -->

    <owl:Class rdf:about="Document">
        <rdfs:label xml:lang="en">Document</rdfs:label>
        <rdfs:comment xml:lang="en"
            >Abstract resource denoting a written document, which may have multiple concrete representations.</rdfs:comment>
    </owl:Class>
    


    <!-- http://id.altlaw.org/vocab/Errata -->

    <owl:Class rdf:about="Errata">
        <rdfs:label xml:lang="en">Errata</rdfs:label>
        <rdfs:subClassOf rdf:resource="Document"/>
        <rdfs:comment xml:lang="en"
            >Document containing a list of errors, corrections, modifications, or additions to another document.</rdfs:comment>
    </owl:Class>
    


    <!-- http://id.altlaw.org/vocab/File -->

    <owl:Class rdf:about="File">
        <rdfs:label xml:lang="en">File</rdfs:label>
        <rdfs:subClassOf rdf:resource="&owl;Thing"/>
        <rdfs:comment xml:lang="en"
            >Concrete binary representation of a Document, such as plain text, HTML, or PDF.</rdfs:comment>
    </owl:Class>
    


    <!-- http://id.altlaw.org/vocab/Order -->

    <owl:Class rdf:about="Order">
        <rdfs:label xml:lang="en">Order</rdfs:label>
        <rdfs:subClassOf rdf:resource="Document"/>
        <rdfs:comment xml:lang="en"
            >Instruction from a court telling some party to do something.</rdfs:comment>
    </owl:Class>
    


    <!-- http://www.w3.org/2002/07/owl#Thing -->

    <owl:Class rdf:about="&owl;Thing"/>
</rdf:RDF>



<!-- Generated by the OWL API (version 2.2.1.1138) http://owlapi.sourceforge.net -->

