<?xml version="1.0" encoding="UTF-8"?>
<!DOCTYPE rdf:RDF [
    <!ENTITY alt "http://id.altlaw.org/terms/">
    <!ENTITY bibo "http://purl.org/ontology/bibo/">
    <!ENTITY dc "http://purl.org/dc/elements/1.1/">
    <!ENTITY dcterms "http://purl.org/dc/terms/">
    <!ENTITY foaf "http://xmlns.com/foaf/0.1/">
    <!ENTITY owl "http://www.w3.org/2002/07/owl#">
    <!ENTITY rdf "http://www.w3.org/1999/02/22-rdf-syntax-ns#">
    <!ENTITY rdfs "http://www.w3.org/2000/01/rdf-schema#">
    <!ENTITY xsd "http://www.w3.org/2001/XMLSchema#">
    <!ENTITY vann "http://purl.org/vocab/vann/">
    <!ENTITY dcdoc "http://dublincore.org/documents/dcmi-terms/">
]>
<rdf:RDF 
    xmlns:alt="&alt;"
    xmlns:bibo="&bibo;"
    xmlns:dcterms="&dcterms;"
    xmlns:foaf="&foaf;"
    xmlns:owl="&owl;"
    xmlns:rdf="&rdf;"
    xmlns:rdfs="&rdfs;"
    xmlns:xsd="&xsd;"
    xmlns:vann="&vann;">


  <!-- The Ontology itself -->

  <owl:Ontology rdf:about="&alt;">
    <rdfs:label>AltLaw.org Vocabulary [DRAFT]</rdfs:label>
    <vann:preferredNamespacePrefix>alt</vann:preferredNamespacePrefix>
    <rdfs:comment>
      An RDF vocabulary for Semantic Web applications using data
      provided by AltLaw.org.  The classes and properties defined here
      are intended to supplement and be used alongside other metadata
      vocabularies such as Dublin Core (&dcterms;) and
      Bibliontology (&bibo;).

      This vocabulary borrows some definitions from the OAI4Courts draft
      specification at
      http://topics.law.cornell.edu/wiki/lexcraft/oai4courts_overview

      This vocabulary redefines some terms that exist in other
      ontologies but are considered "unstable"
      (e.g. "bibo:LegalDecision").

      THIS VOCABULARY IS EXPERIMENTAL AND SUBJECT TO MAJOR CHANGES.

      The RDF/XML source of this vocabulary can be found at
      http://github.com/lawcommons/altlaw-vocab/tree/master/altlaw-vocab.rdf
    </rdfs:comment>
  </owl:Ontology>


  <!-- CLASSES -->

  <owl:Class rdf:about="&alt;Court">
    <rdfs:label>Court</rdfs:label>
    <rdfs:comment>
      Any court.
    </rdfs:comment>
    <rdfs:seeAlso rdf:resource="http://altlaw.org/courts"/>
    <rdfs:subClassOf rdf:resource="&foaf;Organization"/>
    <rdfs:isDefinedBy rdf:resource="&alt;"/>
  </owl:Class>

  <owl:Class rdf:about="&alt;Judgment">
    <rdfs:label>Judgment</rdfs:label>
    <rdfs:comment>
      A determination by a Court on matters put before it.

      A Judgment is an abstract concept, which, when written down,
      becomes a Decision.  However, not all court judgments are
      written down.
    </rdfs:comment>
    <rdfs:isDefinedBy rdf:resource="&alt;"/>
  </owl:Class>

  <owl:Class rdf:about="&alt;Decision">
    <rdfs:label>Decision</rdfs:label>
    <rdfs:comment>
      The written form of a Judgment.  A decision may be a complete
      document in and of itself, or it contain multiple Opinions with
      "dcterms:hasPart".
    </rdfs:comment>
    <owl:equivalentClass rdf:resource="&bibo;LegalDecision"/>
    <rdfs:subClassOf rdf:resource="&bibo;LegalCaseDocument"/>
    <rdfs:subClassOf rdf:resource="&alt;Judgment"/>
    <rdfs:subClassOf>
      <owl:Restriction>
        <owl:allValuesFrom rdf:resource="&alt;Opinion"/>
        <owl:onProperty rdf:resource="&dcterms;hasPart"/>
      </owl:Restriction>
    </rdfs:subClassOf>
    <rdfs:isDefinedBy rdf:resource="&alt;"/>
  </owl:Class>

  <owl:Class rdf:about="&alt;Opinion">
    <rdfs:label>Opinion</rdfs:label>
    <rdfs:comment>
      A single written screed within a Decision.  Represents the view
      of one judge or an agreement among judges, such as a majority
      opinion, concurrence, or dissent.
    </rdfs:comment>
    <rdfs:subClassOf rdf:resource="&bibo;LegalCaseDocument"/>
    <rdfs:subClassOf>
      <owl:Restriction>
        <owl:allValuesFrom rdf:resource="&alt;Decision"/>
        <owl:onProperty rdf:resource="&dcterms;isPartOf"/>
      </owl:Restriction>
    </rdfs:subClassOf>
    <rdfs:isDefinedBy rdf:resource="&alt;"/>
  </owl:Class>

  <owl:Class rdf:about="&alt;BluebookCitation">
    <rdfs:label>BluebookCitation</rdfs:label>
    <rdfs:comment>
      A citation to a document in the form described by "A Uniform
      System of Citation", a.k.a. the Bluebook, available at
      http://www.legalbluebook.com/

      A BluebookCitation is typically composed of a title, one or more
      BluebookLocators, and a year and court in parentheses. Instances
      of this class should have, at a minimum, an rdf:value property
      pointing to the full citation as a string.

      Individual components may be represented by the properties
      dcterms:title, dcterms:date, and alt:court.
      Volume/reporter/page locators may be represented with the
      property dcterms:hasPart pointing to instances of
      BluebookLocator.
    </rdfs:comment>
  </owl:Class>

  <owl:Class rdf:about="&alt;BluebookLocator">
    <rdfs:label>BluebookLocator</rdfs:label>
    <rdfs:comment>
      A Bluebook locator has three parts, as in "[volume] [reporter]
      [page]", with an optional "pincite" giving the page at which a
      particular reference is found.  Instances of this class should
      have, at a minimum, an rdf:value property pointing to the
      locator as a string.  Individual components may be represented
      by the properties bibo:volume, bibo:startPage, and
      dcterms:isPartOf pointing to an instance of bibo:CourtReporter
      or some other collection class.  Pincites may be represented
      with the alt:atPage or alt:atParagraph properties.
    </rdfs:comment>
    <rdfs:isDefinedBy rdf:resource="&alt;"/>
  </owl:Class>

  <owl:Class rdf:about="&alt;Errata">
    <rdfs:label>Errata</rdfs:label>
    <rdfs:comment>
      A document listing corrections, modifications, or additions to
      another document.  We would like to have this in a
      machine-readable form such as a diff, but courts do not publish
      that way.
    </rdfs:comment>
    <rdfs:subClassOf rdf:resource="&bibo;Document"/>
    <rdfs:isDefinedBy rdf:resource="&alt;"/>
  </owl:Class>

  <owl:Class rdf:about="&alt;Process">
    <rdfs:label>Process</rdfs:label>
    <rdfs:comment>
      A single execution of an automated operation, as in a computer.
    </rdfs:comment>
    <rdfs:isDefinedBy rdf:resource="&alt;"/>
  </owl:Class>

  <owl:Class rdf:about="&alt;Crawl">
    <rdfs:label>Crawl</rdfs:label>
    <rdfs:comment>
      A single run of an automated process that retrieves and
      processes Internet resources.
    </rdfs:comment>
    <rdfs:subClassOf rdf:resource="&alt;Process"/>
    <rdfs:isDefinedBy rdf:resource="&alt;"/>
  </owl:Class>

  <owl:Class rdf:about="&alt;Download">
    <rdfs:label>Download</rdfs:label>
    <rdfs:comment>
      Record of downloading a file from an Internet resource.  Used
      for logging HTTP requests/responses.
    </rdfs:comment>
    <rdfs:subClassOf rdf:resource="&alt;Process"/>
    <rdfs:isDefinedBy rdf:resource="&alt;"/>
  </owl:Class>


  <!-- PROPERTIES -->

  <owl:ObjectProperty rdf:about="&alt;court">
    <rdfs:label>court</rdfs:label>
    <rdfs:comment>
      The court associated with a document or event.
    </rdfs:comment>
    <rdfs:subPropertyOf rdf:resource="&dcterms;coverage"/>
    <rdfs:domain rdf:resource="&rdf;Resource"/>
    <rdfs:range rdf:resource="&alt;Court"/>
    <owl:equivalentProperty rdf:resource="&bibo;court"/>
    <rdfs:isDefinedBy rdf:resource="&alt;"/>
  </owl:ObjectProperty>
  
  <owl:DatatypeProperty rdf:about="&alt;documentNumber">
    <rdfs:label>documentNumber</rdfs:label>
    <rdfs:comment>
      The court-assigned document number within a docket.
    </rdfs:comment>
    <rdfs:subPropertyOf rdf:resource="&dcterms;identifier"/>
    <rdfs:domain rdf:resource="&bibo;LegalCaseDocument"/>
    <rdfs:range rdf:resource="&xsd;string"/>
    <rdfs:isDefinedBy rdf:resource="&alt;"/>
  </owl:DatatypeProperty>

  <owl:DatatypeProperty rdf:about="&alt;precedential">
    <rdfs:label>precedential</rdfs:label>
    <rdfs:comment>
      Boolean indicating whether or not a decision is considered
      "precedential" (or, equivalently, "published") by the court that
      issued it.
    </rdfs:comment>
    <rdfs:domain rdf:resource="&alt;Decision"/>
    <rdfs:range rdf:resource="&xsd;boolean"/>
    <rdfs:isDefinedBy rdf:resource="&alt;"/>
  </owl:DatatypeProperty>

  <owl:DatatypeProperty rdf:about="&alt;fullTitle">
    <rdfs:label>fullTitle</rdfs:label>
    <rdfs:comment>
      The full, formal title of the case, e.g. "Oliver Brown et
      al. v. Board of Education of Topeka et al."  A case should have
      only one full title.
    </rdfs:comment>
    <rdfs:domain rdf:resource="&bibo;LegalCaseDocument"/>
    <rdfs:subPropertyOf rdf:resource="&dcterms;title"/>
    <rdfs:isDefinedBy rdf:resource="&alt;"/>
  </owl:DatatypeProperty>

  <owl:DatatypeProperty rdf:about="&alt;shortTitle">
    <rdfs:label>shortTitle</rdfs:label>
    <rdfs:comment>
      A shortened title of a case, as commonly used when citing or
      discussing the case, e.g. "Brown v. Board of Education" or just
      "Brown".  A case may have multiple short titles.
    </rdfs:comment>
    <rdfs:domain rdf:resource="&bibo;LegalCaseDocument"/>

  <owl:DatatypeProperty rdf:about="&alt;gotHttpResponse">
    <rdfs:label>gotHttpResponse</rdfs:label>
    <rdfs:comment>
      A complete log of the HTTP response received from a remote
      server, containing both HTTP headers and entity body.
    </rdfs:comment>
    <rdfs:isDefinedBy rdf:resource="&alt;"/>
    <rdfs:domain rdf:resource="&alt;Download"/>
    <rdfs:range rdf:resource="&xsd;string"/>
  </owl:DatatypeProperty>


  <!-- PROPERTIES DEFINED IN OTHER ONTOLOGIES -->

  <owl:DatatypeProperty rdf:about="&dcterms;date">
    <rdfs:label>dcterms:date</rdfs:label>
    <rdfs:comment>
      The date of a decision.  Use this property only when more
      specific dates, such as "decided" or "issued", are unknown.
      Datatype should be "xsd:date".
    </rdfs:comment>
    <rdfs:seeAlso rdf:resource="&dcdoc;"/>
    <rdfs:isDefinedBy rdf:resource="&dcterms;"/>
    <rdfs:subPropertyOf rdf:resource="&dc;date"/>
  </owl:DatatypeProperty>

  <owl:DatatypeProperty rdf:about="&dcterms;issued">
    <rdfs:label>dcterms:issued</rdfs:label>
    <rdfs:comment>
      The date a Judgment was published.  Use this property only when
      the date of publication is different from the date "decided".
    </rdfs:comment>
    <rdfs:seeAlso rdf:resource="&dcdoc;"/>
    <rdfs:isDefinedBy rdf:resource="&dcterms;"/>
    <rdfs:subPropertyOf rdf:resource="&dcterms;date"/>
  </owl:DatatypeProperty>

  <owl:DatatypeProperty rdf:about="&dcterms;issued">
    <rdfs:label>dcterms:title</rdfs:label>
    <rdfs:comment>
      The title of a case.  Use this property when it is not clear if
      the value represents the full title or a short title.
    </rdfs:comment>
    <rdfs:seeAlso rdf:resource="&dcdoc;"/>
    <rdfs:isDefinedBy rdf:resource="&dcterms;"/>
    <rdfs:subPropertyOf rdf:resource="&dc;title"/>
  </owl:DatatypeProperty>

  <owl:ObjectProperty rdf:about="&dcterms;hasFormat">
    <rdfs:label>dcterms:hasFormat</rdfs:label>
    <rdfs:comment>
      Link to another resource containing the same document in a
      different format.  The target should have a dcterms:format
      property giving its MIME type.
    </rdfs:comment>
    <rdfs:seeAlso rdf:resource="&dcdoc;"/>
    <rdfs:isDefinedBy rdf:resource="&dcterms;"/>
    <rdfs:subPropertyOf rdf:resource="&dcterms;relation"/>
  </owl:ObjectProperty>

  <owl:DatatypeProperty rdf:about="&dcterms;abstract">
    <rdfs:label>dcterms:abstract</rdfs:label>
    <rdfs:comment>
      An abstract or summary of a decision.  Provided by some court
      web sites, but not considered part of the official decision.
    </rdfs:comment>
    <rdfs:seeAlso rdf:resource="&dcdoc;"/>
    <rdfs:isDefinedBy rdf:resource="&dcterms;"/>
    <rdfs:subPropertyOf rdf:resource="&dcterms;description"/>
  </owl:DatatypeProperty>

  <owl:DatatypeProperty rdf:about="&dcterms;subject">
    <rdfs:label>dcterms:subject</rdfs:label>
    <rdfs:comment>
      A keyword or broad topic heading for the case, such as
      "criminal" or "immigration".  Provided by some court web sites,
      but not considered part of the official decision.
    </rdfs:comment>
    <rdfs:seeAlso rdf:resource="&dcdoc;"/>
    <rdfs:isDefinedBy rdf:resource="&dcterms;"/>
    <rdfs:subPropertyOf rdf:resource="&dc;subject"/>
  </owl:DatatypeProperty>

  <owl:DatatypeProperty rdf:about="&dcterms;issued">
    <rdfs:label>dcterms:description</rdfs:label>
    <rdfs:comment>
      Free-text field to store any additional metadata about a case.
      This is where metadata scrapers put any information that they do
      not know how to parse.

      If a scraper knows something about the kind of data the field
      contains, it may prefix the contents with an identifier in ALL
      CAPS, such as "APPEAL FROM" or "HEARD BY".
    </rdfs:comment>
    <rdfs:seeAlso rdf:resource="&dcdoc;"/>
    <rdfs:isDefinedBy rdf:resource="&dcterms;"/>
    <rdfs:subPropertyOf rdf:resource="&dc;description"/>
  </owl:DatatypeProperty>

</rdf:RDF>
