<?xml version="1.0" encoding="UTF-8"?>
<!DOCTYPE rdf:RDF [
    <!ENTITY alt "http://id.altlaw.org/terms/">
    <!ENTITY bibo "http://purl.org/ontology/bibo/">
    <!ENTITY dc "http://purl.org/dc/elements/1.1/">
    <!ENTITY dcterms "http://purl.org/dc/terms/">
    <!ENTITY foaf "http://xmlns.com/foaf/0.1/">
    <!ENTITY owl "http://www.w3.org/2002/07/owl#">
    <!ENTITY rdf "http://www.w3.org/1999/02/22-rdf-syntax-ns#">
    <!ENTITY rdfs "http://www.w3.org/2000/01/rdf-schema#">
    <!ENTITY xsd "http://www.w3.org/2001/XMLSchema#">
    <!ENTITY vann "http://purl.org/vocab/vann/">
    <!ENTITY dcdoc "http://dublincore.org/documents/dcmi-terms/">
    <!ENTITY nfo "http://www.semanticdesktop.org/ontologies/2007/03/22/nfo#">
    <!ENTITY nie "http://www.semanticdesktop.org/ontologies/2007/01/19/nie#">
]>
<rdf:RDF 
    xmlns:alt="&alt;"
    xmlns:bibo="&bibo;"
    xmlns:dc="&dc;"
    xmlns:dcterms="&dcterms;"
    xmlns:foaf="&foaf;"
    xmlns:owl="&owl;"
    xmlns:nfo="&nfo;"
    xmlns:rdf="&rdf;"
    xmlns:rdfs="&rdfs;"
    xmlns:xsd="&xsd;"
    xmlns:vann="&vann;">


  <!-- The Ontology itself -->

  <owl:Ontology rdf:about="&alt;">
    <rdfs:label>AltLaw.org Vocabulary [DRAFT]</rdfs:label>
    <vann:preferredNamespacePrefix>alt</vann:preferredNamespacePrefix>
    <rdfs:comment>
      An RDF vocabulary for Semantic Web applications using data
      provided by AltLaw.org.  Many classes and properties here are
      borrowed directly from Bibliontology, Dublin Core, and the draft
      OAI4Courts specification, with comments indicating how they are
      used by AltLaw.

      THIS VOCABULARY IS EXPERIMENTAL AND SUBJECT TO MAJOR CHANGES.

      The RDF/XML source of this vocabulary can be found at
      http://github.com/lawcommons/altlaw-vocab
    </rdfs:comment>
    <rdfs:seeAlso rdf:resource="&bibo;"/>
    <rdfs:seeAlso rdf:resource="&dcterms;"/>
    <rdfs:seeAlso rdf:resource="http://topics.law.cornell.edu/wiki/lexcraft/oai4courts_overview"/>
  </owl:Ontology>


  <!-- CLASSES -->

  <owl:Class rdf:about="&alt;Court">
    <rdfs:label>alt:Court</rdfs:label>
    <rdfs:comment>
      Any court.
    </rdfs:comment>
    <rdfs:seeAlso rdf:resource="http://altlaw.org/courts"/>
    <rdfs:subClassOf rdf:resource="&foaf;Organization"/>
    <rdfs:isDefinedBy rdf:resource="&alt;"/>
  </owl:Class>

  <owl:Class rdf:about="&alt;Judgment">
    <rdfs:label>alt:Judgment</rdfs:label>
    <rdfs:comment>
      A determination by a Court on matters put before it.

      A Judgment is an abstract concept, the written form of which is
      a bibo:LegalDecision.  However, not all court judgments are
      written down.  Perhaps this should be a parent class of
      bibo:LegalDecision, perhaps the other way around.
    </rdfs:comment>
    <rdfs:isDefinedBy rdf:resource="&alt;"/>
  </owl:Class>

  <owl:Class rdf:abouc="&bibo;LegalDecision">
    <rdfs:label>bibo:LegalDecision</rdfs:label>
    <rdfs:comment>
      A written document containing the authoratitive judgment of a
      court.
    </rdfs:comment>
    <rdfs:isDefinedBy rdf:resource="&bibo;"/>
  </owl:Class>

  <owl:Class rdf:about="&alt;Opinion">
    <rdfs:label>alt:Opinion</rdfs:label>
    <rdfs:comment>
      A single written screed within a court decision.  Represents the
      view of one judge or an agreement among judges, such as a
      majority opinion, concurrence, or dissent.
    </rdfs:comment>
    <rdfs:subClassOf rdf:resource="&bibo;LegalCaseDocument"/>
    <rdfs:subClassOf>
      <owl:Restriction>
        <owl:allValuesFrom rdf:resource="&bibo;LegalDecision"/>
        <owl:onProperty rdf:resource="&dcterms;isPartOf"/>
      </owl:Restriction>
    </rdfs:subClassOf>
    <rdfs:isDefinedBy rdf:resource="&alt;"/>
  </owl:Class>

  <owl:Class rdf:about="&alt;Errata">
    <rdfs:label>alt:Errata</rdfs:label>
    <rdfs:comment>
      A document listing corrections, modifications, or additions to
      another document.  We would like to have this in a
      machine-readable form such as a diff, but courts do not publish
      that way.
    </rdfs:comment>
    <rdfs:subClassOf rdf:resource="&bibo;Document"/>
    <rdfs:isDefinedBy rdf:resource="&alt;"/>
  </owl:Class>


  <!-- PROPERTIES -->

  <!-- Title properties -->

  <owl:DatatypeProperty rdf:about="&alt;fullTitle">
    <rdfs:label>alt:fullTitle</rdfs:label>
    <rdfs:comment>
      The full, formal title of the case, e.g. "Oliver Brown et
      al. v. Board of Education of Topeka et al."  A case should have
      only one full title.  Use "dcterms:title" if uncertain.
    </rdfs:comment>
    <rdfs:domain rdf:resource="&bibo;Document"/>
    <rdfs:subPropertyOf rdf:resource="&dcterms;title"/>
    <rdfs:isDefinedBy rdf:resource="&alt;"/>
  </owl:DatatypeProperty>

  <owl:DatatypeProperty rdf:about="&bibo;shortTitle">
    <rdfs:label>bibo:shortTitle</rdfs:label>
    <rdfs:comment>
      A shortened title of a case, as commonly used when citing or
      discussing the case, e.g. "Brown v. Board of Education" or just
      "Brown".  A case may have multiple short titles.  Use
      "dcterms:title" if uncertain.
    </rdfs:comment>
    <rdfs:isDefinedBy rdf:resource="&bibo;"/>
  </owl:DatatypeProperty>

  <owl:DatatypeProperty rdf:about="&dcterms;issued">
    <rdfs:label>dcterms:title</rdfs:label>
    <rdfs:comment>
      The title of a case.  This property is used when it is not clear
      if the value represents the full title or a short title.
    </rdfs:comment>
    <rdfs:seeAlso rdf:resource="&dcdoc;"/>
    <rdfs:isDefinedBy rdf:resource="&dcterms;"/>
    <rdfs:subPropertyOf rdf:resource="&dc;title"/>
  </owl:DatatypeProperty>


  <!-- Date properties -->

  <owl:DatatypeProperty rdf:about="&dcterms;date">
    <rdfs:label>dcterms:date</rdfs:label>
    <rdfs:comment>
      The principal date of a decision, usually the date it was
      decided.  Datatype should be "xsd:date".
    </rdfs:comment>
    <rdfs:seeAlso rdf:resource="&dcdoc;"/>
    <rdfs:isDefinedBy rdf:resource="&dcterms;"/>
    <rdfs:subPropertyOf rdf:resource="&dc;date"/>
  </owl:DatatypeProperty>


  <!-- Citation properties -->

  <owl:DatatypeProperty rdf:about="&bibo;court">
    <rdfs:label>bibo:court</rdfs:label>
    <rdfs:comment>
      The court associated with a document, such as the court that
      released a decision.
    </rdfs:comment>
    <rdfs:domain rdf:resource="&bibo;LegalDocument"/>
    <rdfs:range rdf:resource="&foaf;Organization"/>
    <rdfs:isDefinedBy rdf:resource="&bibo;"/>
  </owl:DatatypeProperty>

  <owl:DatatypeProperty rdf:about="&alt;bluebookCitation">
    <rdfs:label>alt:blueboookCitation</rdfs:label>
    <rdfs:comment>
      A citation to a document in the form described by "A Uniform
      System of Citation", a.k.a. the Bluebook.  This property refers
      to the complete citation, including title, court, and year.
      Contrast with "alt:bluebookLocator", which contains only the
      volume-series-page portion.
    </rdfs:comment>
    <rdfs:seeAlso rdf:resource="http://www.legalbluebook.com/"/>
    <rdfs:subPropertyOf rdf:resource="&dcterms;identifier"/>
    <rdfs:domain rdf:resource="&bibo;LegalCaseDocument"/>
    <rdfs:range rdf:resource="&xsd;string"/>
    <rdfs:isDefinedBy rdf:resource="&alt;"/>
  </owl:DatatypeProperty>

  <owl:DatatypeProperty rdf:about="&alt;bluebookLocator">
    <rdfs:label>alt:bluebookLocator</rdfs:label>
    <rdfs:comment>
      A Bluebook locator has three parts, as in "[volume] [reporter]
      [page]", with an optional "pincite" giving the page at which a
      particular reference is found.
    </rdfs:comment>
    <rdfs:subPropertyOf rdf:resource="&dcterms;identifier"/>
    <rdfs:domain rdf:resource="&bibo;LegalCaseDocument"/>
    <rdfs:range rdf:resource="&xsd;string"/>
    <rdfs:isDefinedBy rdf:resource="&alt;"/>
  </owl:DatatypeProperty>

  <owl:DatatypeProperty rdf:about="&alt;docketNumber">
    <rdfs:label>alt:docketNumber</rdfs:label>
    <rdfs:comment>
      A court-assigned docket number, sometimes also called a "case
      number."  Value should contain only one docket number, not a
      list of numbers.
    </rdfs:comment>
    <rdfs:subPropertyOf rdf:resource="&dcterms;identifier"/>
    <rdfs:domain rdf:resource="&bibo;LegalCaseDocument"/>
    <rdfs:range rdf:resource="&xsd;string"/>
    <rdfs:isDefinedBy rdf:resource="&alt;"/>
  </owl:DatatypeProperty>

  <owl:DatatypeProperty rdf:about="&alt;documentNumber">
    <rdfs:label>alt:documentNumber</rdfs:label>
    <rdfs:comment>
      The court-assigned document number within a docket.
    </rdfs:comment>
    <rdfs:subPropertyOf rdf:resource="&dcterms;identifier"/>
    <rdfs:domain rdf:resource="&bibo;LegalCaseDocument"/>
    <rdfs:range rdf:resource="&xsd;string"/>
    <rdfs:isDefinedBy rdf:resource="&alt;"/>
  </owl:DatatypeProperty>

  <owl:DatatypeProperty rdf:about="&alt;precedential">
    <rdfs:label>alt:precedential</rdfs:label>
    <rdfs:comment>
      Boolean indicating whether or not a decision is considered
      "precedential" (or, equivalently, "published") by the court that
      issued it.
    </rdfs:comment>
    <rdfs:domain rdf:resource="&bibo;LegalDecision"/>
    <rdfs:range rdf:resource="&xsd;boolean"/>
    <rdfs:isDefinedBy rdf:resource="&alt;"/>
  </owl:DatatypeProperty>


  <!-- File properties -->

  <owl:ObjectProperty rdf:about="&dcterms;hasFormat">
    <rdfs:label>dcterms:hasFormat</rdfs:label>
    <rdfs:comment>
      Link to another resource containing the same document in a
      different format.  The target will have an nie:mimeType
      property giving its MIME type.
    </rdfs:comment>
    <rdfs:seeAlso rdf:resource="&dcdoc;"/>
    <rdfs:isDefinedBy rdf:resource="&dcterms;"/>
    <rdfs:subPropertyOf rdf:resource="&dcterms;relation"/>
  </owl:ObjectProperty>

  <owl:ObjectProperty rdf:about="&nie;mimeType">
    <rdfs:label>nie:mimeType</rdfs:label>
    <rdfs:comment>
      The MIME type of a resource, from the list published by the
      IANA.
    </rdfs:comment>
    <rdfs:seeAlso rdf:resource="http://www.iana.org/assignments/media-types/"/>
    <rdfs:isDefinedBy rdf:resource="&nie;"/>
  </owl:ObjectProperty>


  <!-- Description properties -->

  <owl:ObjectProperty rdf:about="&alt;appealFrom">
    <rdfs:label>alt:appealFrom</rdfs:label>
    <rdfs:comment>
      Link from a LegalDecision to the prior decision or judgment
      being appealed.  Range currently left unspecified, should be
      bibo:LegalDecision or alt:Judgment.
    </rdfs:comment>
    <rdfs:isDefinedBy rdf:resource="&alt;"/>
  </owl:ObjectProperty>

  <owl:DatatypeProperty rdf:about="&dcterms;abstract">
    <rdfs:label>dcterms:abstract</rdfs:label>
    <rdfs:comment>
      An abstract or summary of a decision.  Provided by some court
      web sites, but not considered part of the official decision.
    </rdfs:comment>
    <rdfs:seeAlso rdf:resource="&dcdoc;"/>
    <rdfs:isDefinedBy rdf:resource="&dcterms;"/>
    <rdfs:subPropertyOf rdf:resource="&dcterms;description"/>
  </owl:DatatypeProperty>

  <owl:DatatypeProperty rdf:about="&dcterms;subject">
    <rdfs:label>dcterms:subject</rdfs:label>
    <rdfs:comment>
      A keyword or broad topic heading for the case, such as
      "criminal" or "immigration".  Provided by some court web sites,
      but not considered part of the official decision.
    </rdfs:comment>
    <rdfs:seeAlso rdf:resource="&dcdoc;"/>
    <rdfs:isDefinedBy rdf:resource="&dcterms;"/>
    <rdfs:subPropertyOf rdf:resource="&dc;subject"/>
  </owl:DatatypeProperty>

  <owl:DatatypeProperty rdf:about="&dcterms;issued">
    <rdfs:label>dcterms:description</rdfs:label>
    <rdfs:comment>
      Free-text field to store any additional metadata about a case.
      This is where metadata scrapers put any information that they do
      not know how to parse.

      If a scraper knows something about the kind of data the field
      contains, it may prefix the contents with an identifier in ALL
      CAPS, such as "APPEAL FROM" or "HEARD BY".
    </rdfs:comment>
    <rdfs:seeAlso rdf:resource="&dcdoc;"/>
    <rdfs:isDefinedBy rdf:resource="&dcterms;"/>
    <rdfs:subPropertyOf rdf:resource="&dc;description"/>
  </owl:DatatypeProperty>

</rdf:RDF>
