<?xml version="1.0" encoding="UTF-8"?>
<rdf:RDF 
   xmlns:alt="http://id.altlaw.org/terms/"
   xmlns:bibo="http://purl.org/ontology/bibo/"
   xmlns:dcterms="http://purl.org/dc/terms/"
   xmlns:foaf="http://xmlns.com/foaf/0.1/"
   xmlns:owl="http://www.w3.org/2002/07/owl#"
   xmlns:rdf="http://www.w3.org/1999/02/22-rdf-syntax-ns#"
   xmlns:rdfs="http://www.w3.org/2000/01/rdf-schema#"
   xmlns:xsd="http://www.w3.org/2001/XMLSchema#">


  <!-- The Ontology itself -->

  <owl:Ontology rdf:about="http://id.altlaw.org/terms/">
    <dcterms:title>AltLaw.org Vocabulary</dcterms:title>
    <dcterms:description>
      An RDF vocabulary for Semantic Web applications using data
      provided by AltLaw.org.  The classes and properties defined here
      are intended to supplement and be used alongside other metadata
      vocabularies such as Dublin Core (http://purl.org/dc/terms/) and
      Bibliontology (http://purl.org/ontology/bibo/).

      This ontology borrows some definitions from the OAI4Courts draft
      specification at
      http://topics.law.cornell.edu/wiki/lexcraft/oai4courts_overview

      This ontology redefines some terms that exist in other
      ontologies but are considered "unstable"
      (e.g. "bibo:LegalDecision").
    </dcterms:description>
  </owl:Ontology>


  <!-- CLASSES -->

  <rdfs:Class rdf:about="http://id.altlaw.org/terms/Case">
    <rdfs:label>Case</rdfs:label>
    <rdfs:comment>
      A single dispute among two or more parties.  It may be argued in
      multiple courts at different times, and may result in multiple
      decisions.  Not currently used by AltLaw, but defined in
      OAI4Courts.
    </rdfs:comment>
    <rdfs:isDefinedBy rdf:resource="http://id.altlaw.org/terms/"/>
  </rdfs:Class>

  <rdfs:Class rdf:about="http://id.altlaw.org/terms/Decision">
    <rdfs:label>Decision</rdfs:label>
    <rdfs:comment>
      A single decision released by a court, which may resolve
      multiple cases and contain multiple opinions, concurrences, and
      dissents.  This is the primary type of document handled by
      AltLaw.
    </rdfs:comment>
    <owl:sameAs rdf:resource="http://purl.org/ontology/bibo/LegalDecision"/>
    <rdfs:isDefinedBy rdf:resource="http://id.altlaw.org/terms/"/>
  </rdfs:Class>

  <rdfs:Class rdf:about="http://id.altlaw.org/terms/Opinion">
    <rdfs:label>Opinion</rdfs:label>
    <rdfs:comment>
      A single written screed within a decision.  Represents the view
      of one judge or an agreement among judges, such as a majority
      opinion, concurrence, or dissent.  Not currently used by AltLaw,
      but defined in OAI4Courts.
    </rdfs:comment>
    <rdfs:isDefinedBy rdf:resource="http://id.altlaw.org/terms/"/>
  </rdfs:Class>

  <rdfs:Class rdf:about="http://id.altlaw.org/terms/Court">
    <rdfs:label>Court</rdfs:label>
    <rdfs:comment>
      Any court.  For a list of Semantic Web URIs denoting federal
      courts, see http://altlaw.org/courts
    </rdfs:comment>
    <rdfs:seeAlso rdf:resource="http://altlaw.org/courts"/>
    <rdfs:subClassOf rdf:resource="http://xmlns.com/foaf/0.1/Organization"/>
    <rdfs:isDefinedBy rdf:resource="http://id.altlaw.org/terms/"/>
  </rdfs:Class>

  <rdfs:Class rdf:about="http://id.altlaw.org/terms/File">
    <rdfs:label>File</rdfs:label>
    <rdfs:comment>
      A concrete digital representation of a document.  As opposed to
      the abstract concept of a document and the facts it embodies, a
      File is a sequence of bytes in a particular format and/or
      encoding.  
    </rdfs:comment>
    <rdfs:isDefinedBy rdf:resource="http://id.altlaw.org/terms/"/>
  </rdfs:Class>


  <!-- PROPERTIES -->

  <rdf:Property rdf:about="http://id.altlaw.org/terms/court">
    <rdfs:label>court</rdfs:label>
    <rdfs:comment>
      The court which originated a decision.
    </rdfs:comment>
    <rdfs:subPropertyOf rdf:resource="http://purl.org/dc/terms/coverage"/>
    <rdfs:domain rdf:resource="http://id.altlaw.org/terms/Decision"/>
    <rdfs:range rdf:resource="http://id.altlaw.org/terms/Court"/>
    <owl:sameAs rdf:resource="http://purl.org/ontology/bibo/court"/>
    <rdfs:isDefinedBy rdf:resource="http://id.altlaw.org/terms/"/>
  </rdf:Property>
  
  <rdf:Property rdf:about="http://id.altlaw.org/terms/docket">
    <rdfs:label>docket</rdfs:label>
    <rdfs:comment>
      The docket number associated with a case or decision.  A single
      case or decision may have multiple docket numbers attached to
      it.  The range of this property is any string, which may include
      punctuation such as hyphens, but it should be a single docket
      number rather than a series such as "10-102; 10-103".  The
      string also should not contain abbreviations for "Number" such
      as "No." or "Nos.".
    </rdfs:comment>
    <rdfs:subPropertyOf rdf:resource="http://purl.org/dc/terms/identifier"/>
    <rdfs:range rdf:resource="http://www.w3.org/2000/01/rdf-schema#Literal"/>
    <rdfs:isDefinedBy rdf:resource="http://id.altlaw.org/terms/"/>
  </rdf:Property>

  <rdf:Property rdf:about="http://id.altlaw.org/terms/bluebookIdentifier">
    <rdfs:label>Bluebook identifier</rdfs:label>
    <rdfs:comment>
      A citation to a decision in the form described by "A Uniform
      System of Citation", a.k.a. the Bluebook, available at
      http://www.legalbluebook.com/

      Values of this property should use the three-part syntax
      "[volume] [reporter] [page]".  Additional information such as
      title, date, court, and pinpoint citations ("pincites") should
      be omitted.  Section numbers may be used instead of pages, as in
      "17 U.S.C. &#167; 705".

      A single value of this property must not include parallel
      citations, but a single decision may have multiple
      bluebookIdentifiers, one for each parallel citation.
    </rdfs:comment>
    <rdfs:subPropertyOf rdf:resource="http://purl.org/dc/terms/identifier"/>
    <rdfs:domain rdf:resource="http://id.altlaw.org/terms/Decision"/>
    <rdfs:range rdf:resource="http://www.w3.org/2000/01/rdf-schema#Literal"/>
    <rdfs:isDefinedBy rdf:resource="http://id.altlaw.org/terms/"/>
  </rdf:Property>

  <rdf:Property rdf:about="http://id.altlaw.org/terms/precedential">
    <rdfs:label>precedential</rdfs:label>
    <rdfs:comment>
      Boolean indicating whether or not a decision is considered
      "precedential" (or, equivalently, "published") by the court
      that issued it.  Datatype should be "xsd:boolean".
    </rdfs:comment>
    <rdfs:domain rdf:resource="http://id.altlaw.org/terms/Decision"/>
    <rdfs:range rdf:resource="http://www.w3.org/2000/01/rdf-schema#Literal"/>
    <rdfs:isDefinedBy rdf:resource="http://id.altlaw.org/terms/"/>
  </rdf:Property>

  <rdf:Property rdf:about="http://id.altlaw.org/terms/decided">
    <rdfs:label>decided</rdfs:label>
    <rdfs:comment>
      Date that a court decision/ruling/order was decided.  May or may
      not be the same as date of publication ("dcterms:issued").  This
      is the preferred date to use when describing a court decision.
      Datatype should be "xsd:date".
    </rdfs:comment>
    <rdfs:domain rdf:resource="http://id.altlaw.org/terms/Decision"/>
    <rdfs:range rdf:resource="http://www.w3.org/2000/01/rdf-schema#Literal"/>
    <rdfs:isDefinedBy rdf:resource="http://id.altlaw.org/terms/"/>
  </rdf:Property>

  <rdf:Property rdf:about="http://id.altlaw.org/terms/argued">
    <rdfs:label>argued</rdfs:label>
    <rdfs:comment>
      Date that a case was argued before a court.  Datatype should be
      "xsd:date".
    </rdfs:comment>
    <rdfs:domain rdf:resource="http://id.altlaw.org/terms/Decision"/>
    <rdfs:range rdf:resource="http://www.w3.org/2000/01/rdf-schema#Literal"/>
    <owl:sameAs rdf:resource="http://purl.org/ontology/bibo/argued"/>
    <rdfs:isDefinedBy rdf:resource="http://id.altlaw.org/terms/"/>
  </rdf:Property>

  <rdf:Property rdf:about="http://id.altlaw.org/terms/mimeType">
    <rdfs:label>mimeType</rdfs:label>
    <rdfs:comment>
      The MIME type of a File, a literal string such as
      "application/pdf".  This property is included to avoid potential
      confusion over the correct usage of "dcterms:format", which has
      a non-literal range.
    </rdfs:comment>
    <rdfs:seeAlso rdf:resource="http://www.iana.org/assignments/media-types/"/>
    <rdfs:range rdf:resource="http://www.w3.org/2000/01/rdf-schema#Literal"/>
    <owl:subPropertyOf rdf:resource="http://purl.org/dc/elements/1.1/format"/>
    <rdfs:isDefinedBy rdf:resource="http://id.altlaw.org/terms/"/>
  </rdf:Property>

  <rdf:Property rdf:about="http://id.altlaw.org/terms/charset">
    <rdfs:label>charset</rdfs:label>
    <rdfs:comment>
      The binary character encoding used by a File.  The value of this
      property should be a literal string taken from the list at
      http://www.iana.org/assignments/character-sets

      When a character set has multiple names, the name given as the
      "preferred MIME name" by iana.org should be used.  Preferred
      names for common character sets are "US-ASCII", "ISO-8859-1",
      "windows-1252", and "UTF-8".
    </rdfs:comment>
    <rdfs:seeAlso rdf:resource="http://www.iana.org/assignments/character-sets"/>
    <rdfs:range rdf:resource="http://www.w3.org/2000/01/rdf-schema#Literal"/>
    <owl:subPropertyOf rdf:resource="http://purl.org/dc/elements/1.1/format"/>
    <rdfs:isDefinedBy rdf:resource="http://id.altlaw.org/terms/"/>
  </rdf:Property>



  <!-- PROPERTIES DEFINED IN OTHER ONTOLOGIES -->

  <rdf:Property rdf:about="http://purl.org/dc/terms/date">
    <rdfs:label>dcterms:date</rdfs:label>
    <rdfs:comment>
      The date of a decision.  Use this property only when more
      specific dates, such as "decided" or "issued", are unknown.
      Datatype should be "xsd:date".
    </rdfs:comment>
    <rdfs:isDefinedBy rdf:resource="http://purl.org/dc/terms/"/>
    <owl:subPropertyOf rdf:resource="http://purl.org/dc/elements/1.1/date"/>
  </rdf:Property>

  <rdf:Property rdf:about="http://purl.org/dc/terms/issued">
    <rdfs:label>dcterms:issued</rdfs:label>
    <rdfs:comment>
      The date a decision was published.  Use this property only when
      the date of publication is different from the date "decided".
    </rdfs:comment>
    <rdfs:isDefinedBy rdf:resource="http://purl.org/dc/terms/"/>
    <owl:subPropertyOf rdf:resource="http://purl.org/dc/terms/date"/>
  </rdf:Property>

  <rdf:Property rdf:about="http://purl.org/dc/terms/issued">
    <rdfs:label>dcterms:title</rdfs:label>
    <rdfs:comment>
      The title of a case.  The value of this property should be the
      full, formal title of the case, e.g. "Oliver Brown et
      al. v. Board of Education of Topeka et al."  A case should have
      only one full title.
    </rdfs:comment>
    <rdfs:isDefinedBy rdf:resource="http://purl.org/dc/terms/"/>
    <owl:subPropertyOf rdf:resource="http://purl.org/dc/elements/1.1/title"/>
  </rdf:Property>

  <rdf:Property rdf:about="http://purl.org/ontology/bibo/shortTitle">
    <rdfs:label>bibo:shortTitle</rdfs:label>
    <rdfs:comment>
      A shortened title of a case, as commonly used when citing or
      discussing the case, e.g. "Brown v. Board of Education" or just
      "Brown".  A case may have multiple short titles.
    </rdfs:comment>
    <rdfs:isDefinedBy rdf:resource="http://purl.org/ontology/bibo/"/>
    <owl:subPropertyOf rdf:resource="http://purl.org/dc/terms/alternative"/>
  </rdf:Property>

  <rdf:Property rdf:about="http://purl.org/dc/terms/hasFormat">
    <rdfs:label>dcterms:hasFormat</rdfs:label>
    <rdfs:comment>
      Pointer to a resource containing the content of a decision in
      another format, such as PDF or HTML.  The target resource should
      have a "mimeType" property giving its MIME type.
    </rdfs:comment>
    <rdfs:isDefinedBy rdf:resource="http://purl.org/dc/terms/"/>
    <owl:subPropertyOf rdf:resource="http://purl.org/dc/elements/1.1/relation"/>
  </rdf:Property>

</rdf:RDF>
