<?xml version="1.0" encoding="UTF-8"?>
<rdf:RDF 
   xmlns:alt="http://id.altlaw.org/terms/"
   xmlns:bibo="http://purl.org/ontology/bibo/"
   xmlns:dcterms="http://purl.org/dc/terms/"
   xmlns:foaf="http://xmlns.com/foaf/0.1/"
   xmlns:owl="http://www.w3.org/2002/07/owl#"
   xmlns:rdf="http://www.w3.org/1999/02/22-rdf-syntax-ns#"
   xmlns:rdfs="http://www.w3.org/2000/01/rdf-schema#"
   xmlns:xsd="http://www.w3.org/2001/XMLSchema#">


  <!-- The Ontology itself -->

  <owl:Ontology rdf:about="http://id.altlaw.org/terms/">
    <dcterms:title>AltLaw.org Vocabulary</dcterms:title>
    <dcterms:description>
      An RDF vocabulary for Semantic Web applications using data
      provided by AltLaw.org.  The classes and properties defined here
      are intended to supplement and be used alongside other metadata
      vocabularies such as Dublin Core (http://purl.org/dc/terms/) and
      Bibliontology (http://purl.org/ontology/bibo/).  This ontology
      redefines some terms that exist in other ontologies but are
      considered "unstable" (e.g. "bibo:LegalDecision").
    </dcterms:description>
  </owl:Ontology>


  <!-- CLASSES -->

  <rdfs:Class rdf:about="http://id.altlaw.org/terms/Decision">
    <rdfs:label>Decision</rdfs:label>
    <rdfs:comment>
      A single decision released by a court, which may resolve
      multiple cases and contain multiple writings.
    </rdfs:comment>
    <owl:sameAs rdf:resource="http://purl.org/ontology/bibo/LegalDecision"/>
    <rdfs:isDefinedBy rdf:resource="http://id.altlaw.org/terms/"/>
  </rdfs:Class>

  <rdfs:Class rdf:about="http://id.altlaw.org/terms/Writing">
    <rdfs:label>Writing</rdfs:label>
    <rdfs:comment>
      A single writing within a decision, such as a majority decision,
      concurrence, or dissent.  Not currently used by AltLaw, but
      defined in other vocabularies such as OAI4Courts.
    </rdfs:comment>
    <rdfs:isDefinedBy rdf:resource="http://id.altlaw.org/terms/"/>
  </rdfs:Class>

  <rdfs:Class rdf:about="http://id.altlaw.org/terms/Court">
    <rdfs:label>Court</rdfs:label>
    <rdfs:comment>
      Any court.
    </rdfs:comment>
    <rdfs:subClassOf rdf:resource="http://xmlns.com/foaf/0.1/Organization"/>
    <rdfs:isDefinedBy rdf:resource="http://id.altlaw.org/terms/"/>
  </rdfs:Class>


  <!-- PROPERTIES -->

  <rdf:Property rdf:about="http://id.altlaw.org/terms/court">
    <rdfs:label>court</rdfs:label>
    <rdfs:comment>
      The court which originated a decision.
    </rdfs:comment>
    <rdfs:subPropertyOf rdf:resource="http://purl.org/dc/terms/coverage"/>
    <rdfs:domain rdf:resource="http://id.altlaw.org/terms/Decision"/>
    <rdfs:range rdf:resource="http://id.altlaw.org/terms/Court"/>
    <owl:sameAs rdf:resource="http://purl.org/ontology/bibo/court"/>
    <rdfs:isDefinedBy rdf:resource="http://id.altlaw.org/terms/"/>
  </rdf:Property>
  
  <rdf:Property rdf:about="http://id.altlaw.org/terms/docket">
    <rdfs:label>docket</rdfs:label>
    <rdfs:comment>
      The docket number associated with a case or decision.  A single
      case or decision may have multiple docket numbers attached to
      it.  The range of this property is any string, which may include
      punctuation such as hyphens, but it should be a single docket
      number rather than a series such as "10-102; 10-103".  The
      string also should not contain abbreviations for "Number" such
      as "No." or "Nos.".
    </rdfs:comment>
    <rdfs:subPropertyOf rdf:resource="http://purl.org/dc/terms/identifier"/>
    <rdfs:range rdf:resource="http://www.w3.org/2000/01/rdf-schema#Literal"/>
    <rdfs:isDefinedBy rdf:resource="http://id.altlaw.org/terms/"/>
  </rdf:Property>

  <rdf:Property rdf:about="http://id.altlaw.org/terms/bluebookIdentifier">
    <rdfs:label>Bluebook identifier</rdfs:label>
    <rdfs:comment>
      A citation to a decision in the form described by "A Uniform
      System of Citation", a.k.a. the Bluebook, available at
      http://www.legalbluebook.com/.  Values of this property should
      contain only the minimal information needed to identify the
      decision within a single publication, e.g. "123 F.3d 456".  They
      are not, therefore, complete citations as described by the
      Bluebook.  A single value of this property must not include
      parallel citations, but a single decision may have multiple
      bluebookIdentifiers, one for each parallel citation.
    </rdfs:comment>
    <rdfs:subPropertyOf rdf:resource="http://purl.org/dc/terms/identifier"/>
    <rdfs:domain rdf:resource="http://id.altlaw.org/terms/Decision"/>
    <rdfs:range rdf:resource="http://www.w3.org/2000/01/rdf-schema#Literal"/>
    <rdfs:isDefinedBy rdf:resource="http://id.altlaw.org/terms/"/>
  </rdf:Property>

  <rdf:Property rdf:about="http://id.altlaw.org/terms/precedential">
    <rdfs:label>precedential</rdfs:label>
    <rdfs:comment>
      Boolean indicating whether or not a decision is considered
      "precedential" (or, equivalently, "published") by the court
      that issued it.  Datatype should be "xsd:boolean".
    </rdfs:comment>
    <rdfs:domain rdf:resource="http://id.altlaw.org/terms/Decision"/>
    <rdfs:range rdf:resource="http://www.w3.org/2000/01/rdf-schema#Literal"/>
    <rdfs:isDefinedBy rdf:resource="http://id.altlaw.org/terms/"/>
  </rdf:Property>

  <rdf:Property rdf:about="http://id.altlaw.org/terms/decided">
    <rdfs:label>decided</rdfs:label>
    <rdfs:comment>
      Date that a court decision/ruling/order was decided.  May or may
      not be the same as date of publication ("dcterms:issued").  This
      is the preferred date to use when describing a court decision.
      Datatype should be "xsd:date".
    </rdfs:comment>
    <rdfs:domain rdf:resource="http://id.altlaw.org/terms/Decision"/>
    <rdfs:range rdf:resource="http://www.w3.org/2000/01/rdf-schema#Literal"/>
    <rdfs:isDefinedBy rdf:resource="http://id.altlaw.org/terms/"/>
  </rdf:Property>

  <rdf:Property rdf:about="http://id.altlaw.org/terms/argued">
    <rdfs:label>argued</rdfs:label>
    <rdfs:comment>
      Date that a case was argued before a court.  Refines
      "dcterms:date".  Datatype should be "xsd:date".
    </rdfs:comment>
    <rdfs:domain rdf:resource="http://id.altlaw.org/terms/Decision"/>
    <rdfs:range rdf:resource="http://www.w3.org/2000/01/rdf-schema#Literal"/>
    <owl:sameAs rdf:resource="http://purl.org/ontology/bibo/argued"/>
    <rdfs:isDefinedBy rdf:resource="http://id.altlaw.org/terms/"/>
  </rdf:Property>



  <!-- PROPERTIES DEFINED IN OTHER ONTOLOGIES -->

  <rdf:Property rdf:about="http://purl.org/dc/terms/date">
    <rdfs:label>dcterms:date</rdfs:label>
    <rdfs:comment>
      The date of a decision.  Use this property only when more
      specific dates, such as "decided" or "issued", are unknown.
      Datatype should be "xsd:date".
    </rdfs:comment>
    <rdfs:isDefinedBy rdf:resource="http://purl.org/dc/terms/"/>
    <owl:subPropertyOf rdf:resource="http://purl.org/dc/elements/1.1/date"/>
  </rdf:Property>

  <rdf:Property rdf:about="http://purl.org/dc/terms/issued">
    <rdfs:label>dcterms:issued</rdfs:label>
    <rdfs:comment>
      The date a decision was published.  Use this property only when
      the date of publication is different from the date "decided".
    </rdfs:comment>
    <rdfs:isDefinedBy rdf:resource="http://purl.org/dc/terms/"/>
    <owl:subPropertyOf rdf:resource="http://purl.org/dc/terms/date"/>
  </rdf:Property>

  <rdf:Property rdf:about="http://purl.org/dc/terms/issued">
    <rdfs:label>dcterms:title</rdfs:label>
    <rdfs:comment>
      The title of a case.  The value of this property should be the
      full, formal title of the case, e.g. "Oliver Brown et
      al. v. Board of Education of Topeka et al."  A case should have
      only one full title.
    </rdfs:comment>
    <rdfs:isDefinedBy rdf:resource="http://purl.org/dc/terms/"/>
    <owl:subPropertyOf rdf:resource="http://purl.org/dc/elements/1.1/title"/>
  </rdf:Property>

  <rdf:Property rdf:about="http://purl.org/ontology/bibo/shortTitle">
    <rdfs:comment>
      A shortened title of a case, as commonly used when citing or
      discussing the case, e.g. "Brown v. Board of Education" or just
      "Brown".  A single case may have multiple short titles.
    </rdfs:comment>
    <rdfs:isDefinedBy rdf:resource="http://purl.org/ontology/bibo/"/>
    <owl:subPropertyOf rdf:resource="http://purl.org/dc/terms/alternative"/>
  </rdf:Property>

  <rdf:Property rdf:about="http://purl.org/dc/terms/hasFormat">
    <rdfs:label>dcterms:hasFormat</rdfs:label>
    <rdfs:comment>
      Pointer to a resource containing the content of a decision in
      another format, such as PDF or HTML.  The target resource should
      have a "dcterms:format" property giving its MIME type.
    </rdfs:comment>
    <rdfs:isDefinedBy rdf:resource="http://purl.org/dc/terms/"/>
    <owl:subPropertyOf rdf:resource="http://purl.org/dc/elements/1.1/relation"/>
  </rdf:Property>

  <rdf:Property rdf:about="http://purl.org/dc/terms/format">
    <rdfs:label>dcterms:format</rdfs:label>
    <rdfs:comment>
      The MIME type of a document.  Value should be a literal string
      such as "application/pdf".
    </rdfs:comment>
    <rdfs:seeAlso rdf:resource="http://www.iana.org/assignments/media-types/"/>
    <rdfs:isDefinedBy rdf:resource="http://purl.org/dc/terms/"/>
    <owl:subPropertyOf rdf:resource="http://purl.org/dc/elements/1.1/format"/>
  </rdf:Property>

</rdf:RDF>
